Cleaner DFun (based on DJoin) and clean-up Reprogramming.

DFun.ec
@@ -1,4 +1,4 @@
-require import AllCore List Distr SmtMap FinType DList StdBigop. 
+require import AllCore List Distr DJoin SmtMap FinType StdBigop. 
 (*---*) import Bigreal Bigreal.BRM.
 
 type in_t.
@@ -7,6 +7,7 @@ type out_t.
 clone import FinType as FT_In with
   type t <- in_t.
 
+
 clone import MUniFinFun as MUFF_In with
   type t <- in_t,
   
@@ -14,385 +15,152 @@ clone import MUniFinFun as MUFF_In with
   
   proof *.
 
-(* 
-op doutf : { in_t -> out_t distr | forall (x : in_t), is_lossless (doutf x) } as doutf_ll.
-*)
 
-op [lossless] dout : out_t distr.
-
-clone import DList.Program as DL with
-  type t <- out_t,  
-  op d <- dout.
-
-  
-lemma size_behead (s : 'a list) :
-  size (behead s) = if s = [] then 0 else size s - 1.
-proof. by elim s. qed.
-
-lemma behead_drop (s : 'a list) (i : int)  :
-     0 <= i 
-  => behead (drop i s) = drop (i + 1) s.
-proof.
-elim: s i => [// | x s ih i rng_i].
-case (i = 0) => [-> //= | neq0_i]; 1: by rewrite drop0.
-by rewrite (: ! i <= 0) 2:(: ! i + 1 <= 0) 1,2:/# /= ih // /#.
-qed.
-
-lemma head_drop_nth (x0 : 'a) (s : 'a list) (i : int) :
-     0 <= i < size s
-  => head x0 (drop i s) = nth x0 s i.
-proof.
-elim: s i => [// | x s ih i /= rng_i].
-case (i = 0) => [-> //= | neq0_i].
-by rewrite (: ! i <= 0) 1:/# /= ih /#.
-qed.
-
-lemma uniq_take_drop_mem (x : 'a) (s : 'a list) (i : int) :
-     uniq s
-  => (x \in take i s) 
-  => ! (x \in drop i s).
-proof.
-elim: s i => [// | x' s ih i /= [xpnin uqs]].
-case (i <= 0) => [// | neq0_i].
-case (x = x') => [-> /= | /#].
-by move/contra /(_ xpnin): (mem_drop (i - 1) s x').
-qed.
-
-lemma uniq_drop_take_mem (x : 'a) (s : 'a list) (i : int) :
-     uniq s
-  => (x \in drop i s) 
-  => ! (x \in take i s).
-proof. by smt(uniq_take_drop_mem). qed.
-
-
-lemma uniq_nth (x0 : 'a) (s : 'a list) :
-     uniq s 
-  => (forall (i j : int), 0 <= i < size s => 0 <= j < size s => i <> j =>
-        nth x0 s i <> nth x0 s j).
-proof. by elim: s; smt(nthPn). qed.
-     
-lemma uniq_index_take_mem (x0 x : 'a) (s : 'a list) (i : int) :
-     uniq s
-  => index x s <= i < size s
-  => ! nth x0 s i \in take (index x s) s.
-proof.
-move=> uqs rng_i.
-rewrite (nthPn x0) => j. rewrite size_take 1:index_ge0.
-rewrite (: index x s < size s) 1:/# /=.
-move=> rng_j; rewrite nth_take 1:index_ge0 1:/#.
-by move/uniq_nth /(_ x0 j i _ _): uqs => /#. 
-qed.
-
-lemma eq_from_tofun (s s' : 'a list): 
-     size s = card 
-  => size s' = card 
-  => tofun s = tofun s' 
-  => s = s'.
-proof.
-rewrite /tofun fun_ext => eqsz eqsz' eqf. 
-rewrite &(eq_from_nth witness) // 1:/# => i rng_i.
-move: (eqf (nth witness enum i)).
-by rewrite index_uniq 1:/# 1:enum_uniq.
-qed.
-
-
-op tolist (m : (in_t, out_t) fmap) : (in_t * out_t) list =
-  map (fun x => (x, oget m.[x])) enum.
-
-op tolist_sub (m : (in_t, out_t) fmap) (i : int) : (in_t * out_t) list =
-  map (fun x => (x, oget m.[x])) (take i enum).
-
-lemma tolistsub_empty (m : (in_t, out_t) fmap) (i : int) :
-     i <= 0 
-  => tolist_sub m i = [].
-proof. by move=>?; rewrite /tolist_sub take_le0. qed.
-
-lemma tolistsub_card m :
-  tolist_sub m card = tolist m.
-proof. by rewrite /tolist_sub /tolist take_size. qed.
-
-lemma tolistsubS (m : (in_t, out_t) fmap) (i : int) :
-     0 <= i < card
-  => tolist_sub m (i + 1) 
-     = 
-     rcons (tolist_sub m i) (nth witness enum i, oget m.[nth witness enum i]).
-proof.
-elim; elim: i => [@/tolist_sub /= /# | i ge0_i ih ltc_i1].
-by rewrite {1}/tolist_sub (take_nth witness) 1:/# map_rcons.
-qed.
-
-module Loop_Fmap_Head = {
-  proc sample() : (in_t, out_t) fmap = {
+module Loop_Fmap = {
+  proc sample(d : in_t -> out_t distr, xs : in_t list) : (in_t, out_t) fmap = {
     var m : (in_t, out_t) fmap;
     var x : in_t;
     var y : out_t;
-    var i : int;
-    var w : in_t list;
     
-    w <- enum;
     m <- empty;
-    while (w <> []) {
-      x <- head witness w;
-      y <$ dout;
+    while (xs <> []) {
+      x <- head witness xs;
+      y <$ d x;
       m.[x] <- y;
-      w <- behead w;
-    }
-    
-    return m;    
-  }
-}.
-(*
-module Loop_Fmap_Nth = {
-  proc sample(n : int) : (in_t, out_t) fmap = {
-    var m : (in_t, out_t) fmap;
-    var x : in_t;
-    var y : out_t;
-    var i : int;
-    
-    i <- 0;
-    m <- empty;
-    while (i < n) {
-      x <- nth witness enum i;
-      y <$ dout;
-      m.[x] <- y;
-      i <- i + 1;
+      xs <- behead xs;
     }
     
     return m;    
   }
 }.
 
-module Loop_List_Cons = {
-  proc sample(n : int) : (in_t * out_t) list = {
-    var m : (in_t * out_t) list;
-    var x : in_t;
-    var y : out_t;
-    
-    m <- [];
-    while (size m < n) {
-      x <- nth witness enum (size m);
-      y <$ dout;
-      m <- (x, y) :: m;
-    }
-    
-    return m;    
-  }
-}.
-*)
 module Loop_List_Rcons = {
-  proc sample(n : int) : (in_t * out_t) list = {
+  proc sample(d : in_t -> out_t distr, xs : in_t list) : (in_t * out_t) list = {
     var m : (in_t * out_t) list;
     var x : in_t;
     var y : out_t;
     
     m <- [];
-    while (size m < n) {
-      x <- nth witness enum (size m);
-      y <$ dout;
+    while (xs <> []) {
+      x <- head witness xs;
+      y <$ d x;
       m <- rcons m (x, y);
+      xs <- behead xs;
     }
     
     return m;    
   }
 }.
-
-module Direct = {
-  proc sample() : in_t -> out_t ={
+  
+module Direct_Fun = {
+  proc sample(d : in_t -> out_t distr) : in_t -> out_t ={
     var f : in_t -> out_t;
     
-    f <$ dfun (fun _ => dout);
+    f <$ dfun d;
     
     return f;
   }  
 }.
 
-(*
-equiv Eqv_Loop_Fmap_Head_Nth :
-  Loop_Fmap_Head.sample ~ Loop_Fmap_Nth.sample : n{2} = card ==> ={res}.
+
+
+section.
+
+local equiv Eqv_Loop_Fmap_Loop_List_Rcons :
+  Loop_Fmap.sample ~ Loop_List_Rcons.sample : 
+    ={d, xs} /\ uniq xs{1} 
+    ==>
+    forall (x : in_t), res{1}.[x] = assoc res{2} x. 
 proof.
-proc.
-while (={m} /\ w{1} = drop i{2} enum /\ 0 <= i{2} /\ n{2} = card).
-+ wp; rnd; wp; skip => /> &2 ge0_i neqed ltc_i y yin.
-  by rewrite -nth0_head nth_drop 3:behead_drop //= -size_eq0 size_drop /#.
-wp; skip => />; rewrite drop0; smt(card_gt0).
+proc => /=.
+seq 1 1: (#pre /\ m{1} = empty /\ m{2} = []); 1: by wp.
+exists* xs{2}; elim* => xss.
+while (   ={d, xs}
+       /\ uniq xss 
+       /\ unzip1 m{2} ++ xs{2} = xss
+       /\ #post).
++ wp; rnd; wp; skip => /> &1 &2 uqs eqm neqn_xs y yin.
+  split => [| x]; 1: by rewrite map_rcons /= -cats1 -catA /= head_behead.
+  rewrite -cats1 assoc_cat; case (x = head witness xs{2}) => [-> | neqh_x].
+  - rewrite get_set_sameE (: ! head witness xs{2} \in unzip1 m{2}) /=.
+    *  move/cat_uniq: uqs => [#] _ /hasPn /(_ (head witness xs{2})) + _.
+      by rewrite -(mem_head_behead witness).
+    by rewrite assoc_cons.
+  have eqinx: forall x, x \in m{1} <=> x \in unzip1 m{2}.
+  - move=> x'; split => xpin; move: (eqm x'); apply contraLR => /= xpnin.
+    * by move/domE: xpin => m1nn; move: xpnin; rewrite -assocTP /#.
+    by move/assocTP: xpin => m1nn; move: xpnin; rewrite domE /#.
+  rewrite get_set_neqE //; case: (x \in unzip1 m{2}); 1: by rewrite eqm.
+  by rewrite -eqinx domE /= => ->; rewrite assoc_cons neqh_x assoc_nil.
+by wp; skip => /> &2 uqxs; rewrite emptyE assoc_nil.
 qed.
 
-lemma Eqv_Loop_Fmap_Nth_List_Rcons (_n : int) :
-     0 <= _n <= card
-  => equiv[Loop_Fmap_Nth.sample ~ Loop_List_Rcons.sample : 
-            ={n} /\ n{1} = _n ==> tolist_sub res{1} _n = res{2}].
-proof.
-move=> rng_n.
-proc.
-while (   ={n}
-       /\ n{1} = _n
-       /\ tolist_sub m{1} i{1} = m{2} 
-       /\ i{1} = size m{2}
-       /\ 0 <= i{1} <= n{1}).
-+ wp; rnd; wp; skip => /> &1 eqsz_i ge0_i _ ltn_i ltn_sz y yin.
-  rewrite size_rcons -eqsz_i /=; split => [| /#].
-  rewrite tolistsubS 1:/#; congr. 
-  + rewrite /tolist_sub &(eq_in_map) => x rng_x /=.
-    rewrite get_setE; suff /#: ! (nth witness enum i{1} \in take i{1} enum).
-    rewrite (: i{1} = index (nth witness enum i{1}) enum) 1:index_uniq 1:/# 1:enum_uniq //.
-    by rewrite uniq_index_take_mem 1:enum_uniq // index_mem mem_nth 1:/#. 
-  by rewrite get_set_sameE oget_some.
-by wp; skip => /> /#.
-qed.
-*)
-
-lemma Eqv_Loop_Fmap_Head_List_Rcons (_n : int) :
-     0 <= _n <= card
-  => equiv[Loop_Fmap_Head.sample ~ Loop_List_Rcons.sample : 
-            n{2} = _n ==> tolist_sub res{1} _n = res{2}].
-proof.
-move=> rng_n.
-proc.
-splitwhile{1} 3 : (card - size w < _n).
-while{1} (   tolist_sub m{1} _n = m{2}
-          /\ ! has (mem w{1}) (take _n enum)) (size w{1}).
-+ move => &m z.
-  wp; sp; conseq (: _ ==> true).
-  - move => /> &1 nhas wne y.
-    rewrite size_behead wne /=; split => [| /#].
-    split => [@/tolist_sub |]. 
-    * rewrite -eq_in_map => x xin /=.
-      congr; move/hasPn /(_ x xin): nhas => xnin.  
-      by rewrite get_setE (: x <> head witness w{1}) 1:-nth0_head //; smt(nthPn).
-    by rewrite hasPn => x xin; move/hasPn /(_ x xin): nhas => /#.
-  by rnd; skip; rewrite dout_ll.
-conseq (: _ 
-          ==> 
-             tolist_sub m{1} n{2} = m{2} 
-          /\ ! has (mem w{1}) (take n{2} enum)); 1: smt(size_ge0).
-while (   tolist_sub m{1} (size m{2}) = m{2} 
-       /\ w{1} = drop (size m{2}) enum
-       /\ n{2} = _n
-       /\ card - size w{1} = size m{2}
-       /\ size m{2} <= n{2}).
-+ wp; rnd; wp; skip => |> &1 &2 eqm -> _ dene ltn_szm _ y yin.
-  rewrite size_rcons /= behead_drop 1:/# /=.
-  rewrite size_drop 1:/# -?andbA; split; 2: by smt(size_drop).
-  rewrite tolistsubS 1:/# /=; congr. 
-  - rewrite -{3}eqm /tolist_sub &(eq_in_map) => x rng_x /=.
-    rewrite get_setE head_drop_nth 1:/#. 
-    suff /#: ! (nth witness enum (size m{2}) \in take (size m{2}) enum).
-    rewrite (: (size m{2}) = index (nth witness enum (size m{2})) enum) 1:index_uniq 1:/# 1:enum_uniq //.
-    by rewrite uniq_index_take_mem 1:enum_uniq // index_mem mem_nth 1:/#.
-  by rewrite head_drop_nth 1:/# get_set_sameE oget_some.
-wp; skip => />.
-rewrite tolistsub_empty 2:drop0 //=; split => [/# | m m' *].
-split => [/#| ]; rewrite hasPn => x xin.
-by rewrite (: size m' = _n) 1:/# uniq_take_drop_mem 1:enum_uniq.
-qed.
-
-equiv Eqv_Loop_List_Rcons_Sample:
-  Loop_List_Rcons.sample ~ Sample.sample : ={n} ==> unzip2 res{1} = res{2}.
-proof.
-transitivity LoopSnoc.sample (={n} ==> unzip2 res{1} = res{2}) (={n} ==> ={res}); 1,2: by smt().
-+ proc.
-  while (={n} /\ unzip2 m{1} = l{2} /\ size m{1} = i{2}).
-  - by wp; rnd; wp; skip => />; smt(cats1 map_cat size_rcons).
-  by wp; skip.
-by symmetry; conseq (: ={n} ==> ={res}) => //; apply Sample_LoopSnoc_eq.
-qed.
-
-
-lemma Eqv_Loop_Fmap_Head_Sample (_n : int) :
-     0 <= _n <= card
-  => equiv[Loop_Fmap_Head.sample ~ Sample.sample : 
-        n{2} = _n ==> unzip2 (tolist_sub res{1} _n) = res{2}].
-proof.
-move=> rng_n.
-transitivity Loop_List_Rcons.sample 
-             (n{2} = _n ==> tolist_sub res{1} _n = res{2}) 
-             (={n} ==> unzip2 res{1} = res{2}); 1,2: by smt().
-+ by apply Eqv_Loop_Fmap_Head_List_Rcons.
-by apply Eqv_Loop_List_Rcons_Sample.
-qed.
-
-equiv Eqv_Loop_Fmap_Head_Sample_Card :
-  Loop_Fmap_Head.sample ~ Sample.sample : 
-      n{2} = card ==> unzip2 (tolist res{1}) = res{2}.
-proof.
-conseq (: _ ==> unzip2 (tolist_sub res{1} card) = res{2}) => />.
-+ by move=> r; rewrite tolistsub_card.
-by move: (Eqv_Loop_Fmap_Head_Sample card _); 1: by smt(card_gt0).
-qed.
-
-
-lemma Pr_Sample_offun &m (f : in_t -> out_t) :
-  Pr[Sample.sample(card) @ &m: res = offun f] 
+local lemma Pr_Direct_Fun &m (df : in_t -> out_t distr) (f : in_t -> out_t) :
+  Pr[Direct_Fun.sample(df) @ &m : res = f] 
   = 
-  big predT (fun y => mu1 dout y) (offun f).  
-proof. 
-byphoare (: n = card ==> _) => //.
+  mu1 (dfun df) f.
+proof.
+byphoare (: arg = df ==> res = f) => //.
 proc.
-rnd.
-skip => />.
-rewrite (: (fun (x : out_t list) => x = offun f) = pred1 (offun f)) 1://.    
-rewrite dlist1E; 1: smt(card_gt0). 
-by rewrite size_map /card.
+by rnd; skip.
 qed.
 
+local clone import JoinMapSampling as JMS with
+  type ta <- in_t,
+  type tb <- out_t
+  
+  proof *.
 
-lemma Eq_Pr_Sample_offun_tofun &m (f : in_t -> out_t) :
-  Pr[Sample.sample(card) @ &m: res = offun f] 
+local lemma Pr_S_sample_tofun &m (df : in_t -> out_t distr) (f : in_t -> out_t) :
+  Pr[S.sample(df, enum) @ &m : tofun res = f] 
   = 
-  Pr[Sample.sample(card) @ &m: tofun res = f].    
-proof. 
-byequiv => //.
+  mu1 (dfun df) f.
+proof.
+byphoare (: arg = (df, enum) ==> tofun res = f) => //.
 proc.
-rnd.
-skip => /> r rin.
-by rewrite offunK tofunK; smt(supp_dlist card_gt0).
+rnd; skip => />.
+rewrite (: (fun (x : out_t list) => tofun x = f) = (pred1 f) \o tofun) 1:fun_ext //.
+by rewrite -dfunE_djoin.
 qed.
 
-lemma Pr_Direct &m (f : in_t -> out_t) :
-  Pr[Direct.sample() @ &m : res = f]
-  = 
-  big predT (fun y => mu1 dout y) (offun f). 
+equiv Eqv_Loop_Fmap_Direct_Fun (df : in_t -> out_t distr) :
+  Loop_Fmap.sample ~ Direct_Fun.sample : 
+    arg{1} = (df, enum) /\ arg{2} = df 
+    ==>
+    (fun (x : in_t) => oget res{1}.[x]) = res{2}.
 proof.
-byphoare => //.
-proc. 
-rnd.
-skip => />. 
-by rewrite dfun1E big_mapT.
+transitivity S.sample
+             (={d, xs} /\ xs{1} = enum ==> (fun (x : in_t) => oget res{1}.[x]) = tofun res{2})
+             (arg{1} = (df, enum) /\ arg{2} = df ==> tofun res{1} = res{2}) => //; 1: smt(enum_uniq).
++ transitivity Loop_List_Rcons.sample
+               (={d, xs} /\ uniq xs{1} ==> forall (x : in_t), res{1}.[x] = assoc res{2} x)
+               (={d, xs} /\ xs{1} = enum ==> size res{2} = card /\ res{1} = zip enum res{2}) => //; 1: smt(enum_uniq).
+  - move=> /> &1 &2 eqx eqc.
+    rewrite fun_ext => x; rewrite eqx /tofun.
+    search assoc uniq. search assoc index.
+    rewrite assoc_zip 1:eqc // (onth_nth witness) 2:oget_some //.
+    by rewrite index_ge0 eqc index_mem enumP.
+  - by apply Eqv_Loop_Fmap_Loop_List_Rcons.
+  transitivity S.loop_first
+               (={d, xs} /\ xs{1} = enum ==> size res{2} = card /\ res{1} = zip enum res{2})
+               (={d, xs} ==> ={res}) => //; 1: smt().
+  - proc.
+    while (   ={d, xs} 
+           /\ xs{2} = drop (size l{2}) enum
+           /\ m{1} = zip (take (size l{2}) enum) l{2}
+           /\ size l{2} = card - size xs{2}).
+    * wp; rnd; wp; skip => /> &2 eqszl ^. 
+      rewrite -{1}size_eq0 => neq0_szxs nnxs y yin.
+      rewrite size_rcons; split; 1: by rewrite (drop_nth witness) //; smt(size_ge0).
+      split; last by move: nnxs eqszl; pose xs := drop (size l{2}) enum; case (xs) => // /#.
+      rewrite -zip_rcons 1:size_take; 1,2: smt(size_ge0).
+      by congr; rewrite -nth0_head (take_nth witness) 2:nth_drop //; smt(size_ge0).
+    by wp; skip => />; rewrite drop0 take0 /= => l _ ->; rewrite take_size.
+  - symmetry.
+  conseq (: ={d, xs} ==> ={res}) => //; 1: by smt().
+  by apply Sample_Loop_first_eq.  
+bypr (tofun res{1}) (res{2}) => // /> &1 &2 l -> /= ->.
+by rewrite Pr_Direct_Fun Pr_S_sample_tofun.
 qed.
 
-equiv Eqv_Sample_Direct :
-  Sample.sample ~ Direct.sample: n{1} = card ==> tofun res{1} = res{2}.
-proof.
-bypr (tofun res{1}) (res{2}) => //.
-move => &1 &2 f ->.
-by rewrite -Eq_Pr_Sample_offun_tofun Pr_Sample_offun Pr_Direct.
-qed.
-
-equiv Eqv_Loop_Fmap_Head_Direct :
-  Loop_Fmap_Head.sample ~ Direct.sample : true ==> tofun (unzip2 (tolist res{1})) = res{2}.
-proof.
-transitivity Sample.sample
-             (n{2} = card ==> unzip2 (tolist res{1}) = res{2}) 
-             (n{1} = card ==> tofun res{1} = res{2}); 1,2: smt().
-+ by apply Eqv_Loop_Fmap_Head_Sample_Card.
-by apply Eqv_Sample_Direct.
-qed.
-
-lemma tofun_unzip2_tolist m:
-  tofun (unzip2 (tolist m)) 
-  = 
-  fun (x : in_t) => oget m.[x].
-proof.
-rewrite fun_ext => x @/tofun @/tolist /=.
-rewrite -map_comp /(\o) /=.
-by rewrite (nth_map witness) 2:nth_index // 1:index_ge0 1:index_mem enumP. 
-qed.
-
-equiv Eqv_Loop_Fmap_Head_Direct_Map :
-  Loop_Fmap_Head.sample ~ Direct.sample : 
-    true ==> (fun (x : in_t) => oget res{1}.[x]) = res{2}.
-proof.
-conseq (: _ ==> tofun (unzip2 (tolist res{1})) = res{2}) => />.
-+ by move=> r; rewrite tofun_unzip2_tolist.
-by apply Eqv_Loop_Fmap_Head_Direct.
-qed.
+end section.
