HashFunctionBoundsO.ec
@@ -97,32 +97,6 @@ apply eq_funi_ll; 2,4: by rewrite ?(df_ll, dfc_ll).
 by apply is_full_funiform; 1,2 : rewrite ?(dfc_uni, dfc_fu).
 qed.
 
-(*
-(* 
-  Auxiliary module types for non-keyed hash function properties.
-  Not essential, but used for better readability.
-*)
-module type Oracle_NKi_t = {
-  proc init() : unit
-  proc get(x : input) : output 
-}.
-
-module type Oracle_NK_t = {
-  include Oracle_NKi_t [-init]
-}.
-
-module O_NK_Default : Oracle_NKi_t = {
-  var gk : input -> output
-  
-  proc init() : unit = {
-    gk <$ MUFF_In.dfun (fun _ => doutput);
-  }
-  
-  proc get(x : input) : output = {
-    return gk x;  
-  }
-}.
-*)
 
 (* 
   Auxiliary module for query counting.
@@ -142,7 +116,6 @@ module Counting_O (O : Oracle_t) : Oracle_t = {
 }.
 
 
-
 (* Auxiliary results used in multiple proofs *)
 clone import DMapSampling as DMS with
   type t1 <- (input -> output) * (key -> input -> output),
@@ -158,26 +131,7 @@ module EquivSamplings = {
     
     return g;
   }
-  
-  proc dfc() = {
-    var g : key -> input -> output;
-    
-    g <$ dfc;
-    
-    return g;
-  }
 
-  proc dfc_dep(k : key) = {
-    var gk : input -> output;
-    var g : key -> input -> output;
-    
-    gk <$ dfcs;
-    
-    g <$ dfun kdfcs.[k <- dunit gk];
-    
-    return g;    
-  }
-  
   proc dfc_indep(k : key) = {
     var gk : input -> output;
     var g : key -> input -> output;
@@ -240,50 +194,9 @@ rnd : *0 *0.
 skip => />.
 by rewrite dmap_id.
 qed.
-(*
-equiv Eqv_fixone_if_dfc :
-  EquivSamplings.fixone_dfc ~ EquivSamplings.if_dfc : ={k} ==> ={res}.
-proof.
-proc.
-pose d := dlet dfcs (fun gk => dmap dfc (fun g => (gk, g))).
-transitivity{1} {g <@ S.sample(d, fun (gkg : _ * _) (k' : key) => 
-                                    if k' = k then gkg.`1 else gkg.`2 k'); }
-                (={k} ==> ={g})
-                (={k} ==> g{1} = fun k' => if k' = k{2} then gk{2} else g{2} k'); 1,2: by smt().
-+ inline *.
-  wp; sp.
-  rnd : *0 *0.
-  skip => /> &2; rewrite ?dmap_id.
-  split => [g gin | h g].
-  - congr => @/d.
-    rewrite dmap_dlet /=; congr.
-    rewrite fun_ext => gk.
-    rewrite dmap_comp /(\o) dmap_id /dfc /"_.[_<-_]".
-    rewrite (MUFF_Key.dmap_dfun _ (fun k' f => if k' = k{2} then gk else f)) /=.
-    congr; rewrite fun_ext => k'.
-    case (k{2} = k') => [->|] /=; 1: by rewrite dmap_cst 1:dfcs_ll.
-    by rewrite eq_sym => -> /=; rewrite dmap_id.
-  rewrite supp_dlet => -[gk [gkin /=]]; rewrite supp_dmap => -[gfix [+ ->] /=]. 
-  rewrite dfun_supp supp_dmap => gfixin; exists (gk, gfix); split => /=.
-  + rewrite /d supp_dlet; exists gk; rewrite gkin /= supp_dmap.
-    by exists gfix; rewrite dfc_fu. 
-  rewrite fun_ext => k'; move: (gfixin k').
-  rewrite  /"_.[_<-_]" /=; case (k' = k{2}) => [-> /=|]; 1: by rewrite supp_dunit.
-  by rewrite eq_sym.
-transitivity{1} {g <@ S.map(d, fun (gkg : _ * _) (k' : key) => 
-                                    if k' = k then gkg.`1 else gkg.`2 k'); }
-                (={k} ==> ={g})
-                (={k} ==> g{1} = fun k' => if k' = k{2} then gk{2} else g{2} k'); 1,2: by smt().
-+ by call sample.
-inline *.
-wp; sp.
-rnd : *0 *0.
-skip => />.
-by rewrite dmap_id.
-qed.
-*)
 
 
+(** Bound for SPR **)
 theory SPRBound.
 
 op [lossless] dkey : key distr.
@@ -296,9 +209,6 @@ clone import SPR as KHFO_SPR with
   proof *.
   realize din_ll by exact: dinput_ll.
   realize dkey_ll by exact: dkey_ll.
-
-
-print BFOF.
 
 module (R_BFFind_SPR (A : Adv_SPR) : Adv_BFFind) (BFO : BFOF_t) = {
   var k0 : key
@@ -343,269 +253,6 @@ module (R_BFFind_SPR (A : Adv_SPR) : Adv_BFFind) (BFO : BFOF_t) = {
 section.
 
 declare module A <: Adv_SPR {-KHFO.O_Default, -R_BFFind_SPR, -BFOF, -BFOD}.
-(*
-local module SPR_SS = {
-  var k0 : key
-  var g : key -> input -> output
-  
-  module O_SPR_SS : Oracle_t = {
-    proc get(k : key, x : input) = {
-      
-      return g k x;
-    }
-  }
-  
-  proc main() : bool = {
-    var gk : input -> output;
-    var x, x' : input;
-    var y, y' : output;
-    
-    k0 <$ dkey;
-    
-    gk <$ dfcs;
-    g <$ dfc;
-    
-    x <$ dinput;
-    y <@ O_SPR_SS.get(k0, x);
-    
-    x' <@ A(O_SPR_SS).find(k0, x);
-    y' <@ O_SPR_SS.get(k0, x');
-    
-    return x' <> x /\ y' = y;
-  }
-}.
-*)
-
-(*
-local module SPR_SS = {
-  var k0 : key
-  var g : key -> input -> output
-  
-  module O_SPR_SS : Oracle_t = {
-    proc get(k : key, x : input) = {
-      return g k x;
-    }
-  }
-  
-  proc main() : bool = {
-    var gk : input -> output;
-    var x, x' : input;
-    var y, y' : output;
-    
-    k0 <$ dkey;
-    
-    gk <$ dfcs;
-    g <$ dfun kdfcs.[k0 <- dunit gk];
-    
-    x <$ dinput;
-    y <@ O_SPR_SS.get(k0, x);
-    
-    x' <@ A(O_SPR_SS).find(k0, x);
-    y' <@ O_SPR_SS.get(k0, x');
-    
-    return x' <> x /\ y' = y;
-  }
-}.
-
-local lemma EqPr_SPR_SPRSS &m:
-  Pr[SPR(A, O_Default).main() @ &m : res]
-  =
-  Pr[SPR_SS.main() @ &m : res].
-proof.
-byequiv => //=.
-proc; inline *.
-swap{1} 2 -1.
-seq 1 1 : (={glob A} /\ k{1} = SPR_SS.k0{2}); 1: by rnd.
-wp.
-conseq (: _ ==>    ={x, x', y} 
-                /\ k{1} = SPR_SS.k0{2} 
-                /\ O_Default.f{1} = SPR_SS.g{2}); 1: by smt().
-call (: O_Default.f{1} = SPR_SS.g{2}); 1: by proc.
-wp; rnd => />; 1: by smt().
-transitivity{1} {O_Default.f <$ dfc;}
-                (true ==> ={O_Default.f})
-                (true ==>  O_Default.f{1} = SPR_SS.g{2}) => //.
-+ by rnd; skip => />; rewrite eq_df_dfc.
-rnd: *0 *0.
-wp; skip => /> &2.
-split => [g gin | eqmug f fin].
-+ rewrite dmap_id; congr.
-  rewrite /dfc (MUFF_Key.dfunE_dlet_fix1 _ (SPR_SS.k0{2})) /=.
-  by rewrite /dfcs /kdfcs /dfcs; congr; rewrite fun_ext => f; rewrite dmap_id.
-rewrite supp_dlet /=; exists (f SPR_SS.k0{2}).
-split; 1: by rewrite dfun_fu /= 1:dunifin_fu dmap_id //= dfun_fu.
-rewrite dmap_id dfun_supp => k @/Logic."_.[_<-_]". 
-case (SPR_SS.k0{2} = k) => [-> | ?]; 1: by rewrite supp_dunit.
-by rewrite dmap_id dfun_supp in fin => /#.
-qed.
-
-local lemma EqPr_SPRSS_SPRNK &m:
-  Pr[SPR_SS.main() @ &m : res]
-  =
-  Pr[SPR_NK(R_SPRNK_SPR(A), O_NK_Default).main() @ &m : res].
-proof.
-byequiv=> //=.
-proc; inline *.
-swap{2} 6 -5; swap{2} 7 -4.
-seq 3 3 : (   ={glob A} 
-           /\ ={k0}(SPR_SS, R_SPRNK_SPR)
-           /\ SPR_SS.O_SPR_SS.g{1} 
-              = 
-              (fun k => 
-                if k = R_SPRNK_SPR.k0{2}
-                then O_NK_Default.gk{2}
-                else R_SPRNK_SPR.g{2} k)).
-+ seq 1 1 : (={glob A} /\ ={k0}(SPR_SS, R_SPRNK_SPR)); 1: by rnd.
-  conseq (: _ ==> SPR_SS.O_SPR_SS.g{1} 
-                  =
-                  fun (k : key) =>
-                    if k = R_SPRNK_SPR.k0{2} 
-                    then O_NK_Default.gk{2}
-                    else R_SPRNK_SPR.g{2} k) => //.
-  transitivity{1} {SPR_SS.O_SPR_SS.g <@ EquivSamplings.fixone_dfc(SPR_SS.k0);}
-                  (={SPR_SS.k0} ==> ={SPR_SS.O_SPR_SS.g})
-                  (SPR_SS.k0{1} = R_SPRNK_SPR.k0{2} 
-                   ==> 
-                   SPR_SS.O_SPR_SS.g{1}
-                   = 
-                   (fun k =>  
-                     if k = R_SPRNK_SPR.k0{2}
-                     then O_NK_Default.gk{2}
-                     else R_SPRNK_SPR.g{2} k)); 1,2: by smt().
-  - inline *.
-    wp; sp.
-    rnd; rnd.
-    by skip.
-  transitivity{1} {SPR_SS.O_SPR_SS.g <@ EquivSamplings.if_dfc(SPR_SS.k0);}
-                  (={SPR_SS.k0} ==> ={SPR_SS.O_SPR_SS.g})
-                  (SPR_SS.k0{1} = R_SPRNK_SPR.k0{2} 
-                   ==> 
-                   SPR_SS.O_SPR_SS.g{1}
-                   = 
-                   (fun k =>  
-                     if k = R_SPRNK_SPR.k0{2}
-                     then O_NK_Default.gk{2}
-                     else R_SPRNK_SPR.g{2} k)); 1,2: by smt().
-  - by call Eqv_fixone_if_dfc.
-  inline *.
-  wp; sp.
-  rnd; rnd.
-  by skip.
-wp.
-call (:   SPR_SS.k0{1} = R_SPRNK_SPR.k0{2} 
-       /\ SPR_SS.O_SPR_SS.g{1} 
-          =
-          (fun (k : key) =>
-            if k = R_SPRNK_SPR.k0{2}
-            then O_NK_Default.gk{2}
-            else R_SPRNK_SPR.g{2} k)).
-+ proc; inline *.
-  by wp; skip.
-by wp; rnd; skip.
-qed.
-
-
-local module SPR_NK_Rep (A : Adv_SPR_NK) = {
-  var x0 : input
-  var y0 : output
-  var f : input -> output
-  
-  module O_SPR_NK_Rep : Oracle_NK_t = {
-    proc get(x : input) : output = {
-      var b;
-      
-      b <@ BFOF.query(x);
-      
-      return if !b /\ x <> x0 then f x else y0;
-    }
-  }
-
-  proc main() : bool = {
-    var x' : input;
-    var y' : output;
-    
-    BFOF.init();
-
-    x0 <$ dinput;
-    y0 <$ doutput;
-
-    f <$ MUFF_In.dfun (fun _ => doutput \ (pred1 y0));    
-    
-    x' <@ A(O_SPR_NK_Rep).find(x0);
-    
-    y' <@ O_SPR_NK_Rep.get(x');
-    
-    return x' <> x0 /\ y' = y0;
-  }
-}.
-
-local lemma EqPr_SPRNK_SPRNKRep &m :
-  Pr[SPR_NK(R_SPRNK_SPR(A), O_NK_Default).main() @ &m : res]
-  =
-  Pr[SPR_NK_Rep(R_SPRNK_SPR(A)).main() @ &m : res].
-proof.
-byequiv=> //=.
-proc; inline *.
-wp.
-call (: ={R_SPRNK_SPR.k0, R_SPRNK_SPR.g} /\
-        (forall (x : input), 
-          O_NK_Default.gk{1} x 
-          = 
-          if !BFOF.f{2} x /\ x <> SPR_NK_Rep.x0{2} 
-          then SPR_NK_Rep.f{2} x 
-          else SPR_NK_Rep.y0{2})).
-+ by proc; inline *; auto => /> &1 &2 /(_ x{2}).
-rnd; rnd; wp.
-swap{1} 2 -1; swap{2} 2 -1.
-seq 1 1 : (={glob A} /\ x{1} = SPR_NK_Rep.x0{2}); 1: by rnd.
-conseq (_ : _ 
-            ==> 
-            (forall (x : input), 
-              O_NK_Default.gk{1} x 
-              = 
-              if !BFOF.f{2} x /\ x <> SPR_NK_Rep.x0{2} 
-              then SPR_NK_Rep.f{2} x 
-              else SPR_NK_Rep.y0{2})).
-+ move=> /> &2 gk fl y0 br ih k kin gL glin r.
-  by rewrite (eq_sym r); congr; rewrite !ih //= /#.
-transitivity{1} {O_NK_Default.gk <@ LR.LambdaRepro.left();}
-                (true ==> ={O_NK_Default.gk})
-                (x{1} = SPR_NK_Rep.x0{2} 
-                 ==> 
-                 (forall (x : input),
-                   O_NK_Default.gk{1} x 
-                   =
-                   if ! BFOF.f{2} x /\ x <> SPR_NK_Rep.x0{2} 
-                   then SPR_NK_Rep.f{2} x
-                   else SPR_NK_Rep.y0{2})); 1,2: by smt().
-+ inline *.
-  by wp; rnd.
-transitivity{1} {O_NK_Default.gk <@ LR.LambdaRepro.right(x);}
-                (true ==> ={O_NK_Default.gk})
-                (x{1} = SPR_NK_Rep.x0{2} 
-                 ==> 
-                 (forall (x : input),
-                   O_NK_Default.gk{1} x 
-                   =
-                   if ! BFOF.f{2} x /\ x <> SPR_NK_Rep.x0{2} 
-                   then SPR_NK_Rep.f{2} x
-                   else SPR_NK_Rep.y0{2})); 1,2: by smt().
-+ by call LR.main_theorem.
-inline *.
-wp; rnd.
-swap{2} 1 1.
-by rnd; rnd; wp; skip.
-qed.  
-
-
-local lemma EqPr_SPR_SPRNKRep &m:
-  Pr[SPR(A, O_Default).main() @ &m : res]
-  =
-  Pr[SPR_NK_Rep(R_SPRNK_SPR(A)).main() @ &m : res].
-proof. 
-by rewrite EqPr_SPR_SPRSS EqPr_SPRSS_SPRNK EqPr_SPRNK_SPRNKRep. 
-qed.
-*)
 
 local lemma SPR_Implies_BFFind &m :
   Pr[KHFO_SPR.SPR(A, KHFO.O_Default).main() @ &m : res] 
@@ -632,13 +279,13 @@ seq 1 4 : (   #pre
 + conseq (: true 
             ==>
                (forall (k : key, x : input),
-                   O_Default.f{1} k x
-                   =
-                   if k = R_BFFind_SPR.k0{2}
-                   then (if !BFOF.f{2} x /\ x <> R_BFFind_SPR.x0{2} 
-                        then R_BFFind_SPR.gk{2} x 
-                        else R_BFFind_SPR.y0{2})
-                   else R_BFFind_SPR.g{2} k x)
+                 O_Default.f{1} k x
+                 =
+                 if k = R_BFFind_SPR.k0{2}
+                 then (if !BFOF.f{2} x /\ x <> R_BFFind_SPR.x0{2} 
+                      then R_BFFind_SPR.gk{2} x 
+                      else R_BFFind_SPR.y0{2})
+                 else R_BFFind_SPR.g{2} k x)
             /\ (forall (x : input),
                  R_BFFind_SPR.gk{2} x <> R_BFFind_SPR.y0{2})) => //.
   transitivity{1} {O_Default.f <@ EquivSamplings.df();}
@@ -654,7 +301,7 @@ seq 1 4 : (   #pre
                             else R_BFFind_SPR.y0{2})
                        else R_BFFind_SPR.g{2} k x)
                    /\ (forall (x : input),
-                         R_BFFind_SPR.gk{2} x <> R_BFFind_SPR.y0{2})); 1,2: smt().
+                        R_BFFind_SPR.gk{2} x <> R_BFFind_SPR.y0{2})); 1,2: smt().
   - inline *.
     by wp; rnd.
   transitivity{1} {O_Default.f <@ EquivSamplings.dfc_indep(k);}
@@ -673,20 +320,49 @@ seq 1 4 : (   #pre
                          R_BFFind_SPR.gk{2} x <> R_BFFind_SPR.y0{2})); 1,2: smt().
   - by call Eqv_df_dfc_indep.
   inline *.
-  wp; sp.
-  seq 1 3 : (   #pre
-             /\ (forall (x : input), 
-                   gk{1} x 
-                   =
-                   if !BFOF.f{2} x /\ x <> R_BFFind_SPR.x0{2} 
-                   then R_BFFind_SPR.gk{2} x 
-                   else R_BFFind_SPR.y0{2})
-             /\ (forall (x : input),
-                   R_BFFind_SPR.gk{2} x <> R_BFFind_SPR.y0{2})).
-                   admit.
+  wp; sp => />.
+seq 1 3 : (   (forall (x : input), 
+                 gk{1} x 
+                 =
+                 if !BFOF.f{2} x /\ x <> R_BFFind_SPR.x0{2} 
+                 then R_BFFind_SPR.gk{2} x 
+                 else R_BFFind_SPR.y0{2})
+           /\ (forall (x : input),
+                 R_BFFind_SPR.gk{2} x <> R_BFFind_SPR.y0{2})); last first.
   - by rnd; skip => /> /#.
-sp.
-call (:  (forall (k : key, x : input),
+  transitivity{1} {gk <@ LR.LambdaRepro.left();}
+                (true ==> ={gk})
+                (true 
+                 ==> 
+                    (forall (x : input),
+                       gk{1} x 
+                       =
+                       if ! BFOF.f{2} x /\ x <> R_BFFind_SPR.x0{2} 
+                       then R_BFFind_SPR.gk{2} x
+                       else R_BFFind_SPR.y0{2})
+                 /\ (forall (x : input),
+                       R_BFFind_SPR.gk{2} x <> R_BFFind_SPR.y0{2})); 1,2: smt().
+  - inline *.
+    by wp; rnd.
+  transitivity{1} {gk <@ LR.LambdaRepro.right(x);}
+                  (true ==> ={gk})
+                  (x{1} = R_BFFind_SPR.x0{2} 
+                   ==> 
+                     (forall (x : input),
+                         gk{1} x 
+                         =
+                         if ! BFOF.f{2} x /\ x <> R_BFFind_SPR.x0{2} 
+                         then R_BFFind_SPR.gk{2} x
+                         else R_BFFind_SPR.y0{2})
+                   /\ (forall (x : input),
+                         R_BFFind_SPR.gk{2} x <> R_BFFind_SPR.y0{2})); 1,2: smt().
+  - by call LR.main_theorem.
+  inline *.
+  wp; sp => /=.
+  swap{1} 1 1.
+  rnd; rnd; rnd; skip => /> ? ? ? ? ? ? _ /dfun_supp + x.
+  by move => /(_ x) /= /supp_dexcepted [@/pred1].
+call (: (forall (k : key, x : input),
            O_Default.f{1} k x
            =
            if k = R_BFFind_SPR.k0{2}
@@ -696,7 +372,7 @@ call (:  (forall (k : key, x : input),
            else R_BFFind_SPR.g{2} k x)).
 + proc; inline *.
   by wp; skip => /> /#.
-by skip => /> /#.
+by wp; skip => /> /#.
 qed.
 
 local lemma SPR_Implies_BFDistinguish &m:
@@ -715,989 +391,7 @@ end section.
 end SPRBound.
 
 
-(* 
-  Definitions concerning SPR for non-keyed functions.
-  Used as intermediate step; could inline reduction
-  to remove all these extra definitions (but makes reduction
-  bit less readable).
-
-module type Adv_SPR_NK (O : Oracle_NK_t) = {
-  proc find(x : input) : input
-}.
-
-module SPR_NK (A : Adv_SPR_NK) (O : Oracle_NKi_t) = {
-  proc main() : bool = {
-    var x, x' : input;
-    var y, y' : output;
-    
-    O.init();
-    
-    x <$ dinput;
-    
-    y <@ O.get(x);
-    
-    x' <@ A(O).find(x);
-    
-    y' <@ O.get(x');
-    
-    return x' <> x /\ y' = y;
-  }
-}.
-
-module (R_SPRNK_SPR (A : Adv_SPR) : Adv_SPR_NK) (O : Oracle_NK_t) = {
-  var k0 : key
-  var g : key -> input -> output
-  
-  module O_R_SPRNK_SPR : Oracle_t = {
-    proc get(k : key, x : input) : output = {
-      var y : output;
-      
-      if (k = k0) {
-        y <@ O.get(x);  
-      } else {
-        y <- g k x;
-      }
-      
-      return y;
-    }
-  }
-  
-  proc find(x : input) : input = {
-    var x' : input;
-    
-    k0 <$ dkey;
-    
-    g <$ dfc;
-    
-    x' <@ A(O_R_SPRNK_SPR).find(k0, x);
-     
-    return x';
-  } 
-}.
-
-module (R_BFFind_SPRNK (A : Adv_SPR) : Adv_BFFind) (BFO : BFOF_t) = {
-  var f : input -> output
-  var x0 : input
-  var y0 : output
-  
-  module O_R_BFFind_SPRNK : Oracle_NK_t = {
-    proc get(x : input) : output = {
-      var b : bool;
-      var y : output;
-      
-      b <@ BFO.query(x);
-     
-      return if !b /\ x <> x0 then f x else y0;
-    }
-  }
-
-  proc find() : input = {
-    var x' : input;
-    
-    x0 <$ dinput;
-    y0 <$ doutput;
-    
-    f <$ dfun (fun (_ : input) => doutput \ (pred1 y0));
-            
-    x' <@ R_SPRNK_SPR(A, O_R_BFFind_SPRNK).find(x0);
-    
-    return x';
-  }
-}.
-
-
-section.
-
-declare module A <: Adv_SPR {-KHFO.O_Default, -R_BFFind_SPRNK, -O_NK_Default, -BFOF, -BFOD}.
-
-local module SPR_SS = {
-  var k0 : key
-  
-  module O_SPR_SS : Oracle_t = {  
-    var g : key -> input -> output
-    
-    proc init() : unit = {
-      var gk : input -> output;
-      
-      gk <$ dfcs;
-      
-      g <$ dfun kdfcs.[k0 <- dunit gk];
-    }
-    
-    proc get(k : key, x : input) = {
-      return g k x;
-    }
-  }
-  
-  proc main() : bool = {
-    var x, x' : input;
-    var y, y' : output;
-    
-    k0 <$ dkey;
-    
-    O_SPR_SS.init();
-    
-    x <$ dinput;
-    y <@ O_SPR_SS.get(k0, x);
-    
-    x' <@ A(O_SPR_SS).find(k0, x);
-    y' <@ O_SPR_SS.get(k0, x');
-    
-    return x' <> x /\ y' = y;
-  }
-}.
-
-local lemma EqPr_SPR_SPRSS &m:
-  Pr[SPR(A, O_Default).main() @ &m : res]
-  =
-  Pr[SPR_SS.main() @ &m : res].
-proof.
-byequiv => //=.
-proc; inline *.
-swap{1} 2 -1.
-seq 1 1: (={glob A} /\ k{1} = SPR_SS.k0{2}); 1: by rnd.
-wp.
-conseq (: _ ==>    ={x, x', y} 
-                /\ k{1} = SPR_SS.k0{2} 
-                /\ O_Default.f{1} = SPR_SS.O_SPR_SS.g{2}); 1: by smt().
-call (: O_Default.f{1} = SPR_SS.O_SPR_SS.g{2}); 1: by proc.
-wp; rnd => />; 1: by smt().
-transitivity{1} {O_Default.f <$ dfc;}
-                (true ==> ={O_Default.f})
-                (true ==>  O_Default.f{1} = SPR_SS.O_SPR_SS.g{2}) => //.
-+ by rnd; skip => />; rewrite eq_df_dfc.
-rnd: *0 *0.       
-wp; skip => /> &2.
-split => [g gin | eqmug f fin].
-+ rewrite dmap_id; congr.
-  rewrite /dfc (MUFF_Key.dfunE_dlet_fix1 _ (SPR_SS.k0{2})) /=.
-  by rewrite /dfcs /kdfcs /dfcs; congr; rewrite fun_ext => f; rewrite dmap_id.
-rewrite supp_dlet /=; exists (f SPR_SS.k0{2}).
-split; 1: by rewrite dfun_fu /= 1:dunifin_fu dmap_id //= dfun_fu.
-rewrite dmap_id dfun_supp => k @/Logic."_.[_<-_]". 
-case (SPR_SS.k0{2} = k) => [-> | ?]; 1: by rewrite supp_dunit.
-by rewrite dmap_id dfun_supp in fin => /#.
-qed.
-
-local lemma EqPr_SPRSS_SPRNK &m:
-  Pr[SPR_SS.main() @ &m : res]
-  =
-  Pr[SPR_NK(R_SPRNK_SPR(A), O_NK_Default).main() @ &m : res].
-proof.
-byequiv=> //=.
-proc; inline *.
-swap{2} 6 -5; swap{2} 7 -4.
-seq 3 3 : (   ={glob A} 
-           /\ ={k0}(SPR_SS, R_SPRNK_SPR)
-           /\ SPR_SS.O_SPR_SS.g{1} 
-              = 
-              (fun k => 
-                if k = R_SPRNK_SPR.k0{2}
-                then O_NK_Default.gk{2}
-                else R_SPRNK_SPR.g{2} k)).
-+ seq 1 1 : (={glob A} /\ ={k0}(SPR_SS, R_SPRNK_SPR)); 1: by rnd.
-  conseq (: _ ==> SPR_SS.O_SPR_SS.g{1} 
-                  =
-                  fun (k : key) =>
-                    if k = R_SPRNK_SPR.k0{2} 
-                    then O_NK_Default.gk{2}
-                    else R_SPRNK_SPR.g{2} k) => //.
-  transitivity{1} {SPR_SS.O_SPR_SS.g <@ EquivSamplings.fixone_dfc(SPR_SS.k0);}
-                  (={SPR_SS.k0} ==> ={SPR_SS.O_SPR_SS.g})
-                  (SPR_SS.k0{1} = R_SPRNK_SPR.k0{2} 
-                   ==> 
-                   SPR_SS.O_SPR_SS.g{1}
-                   = 
-                   (fun k =>  
-                     if k = R_SPRNK_SPR.k0{2}
-                     then O_NK_Default.gk{2}
-                     else R_SPRNK_SPR.g{2} k)); 1,2: by smt().
-  - inline *.
-    wp; sp.
-    rnd; rnd.
-    by skip.
-  transitivity{1} {SPR_SS.O_SPR_SS.g <@ EquivSamplings.if_dfc(SPR_SS.k0);}
-                  (={SPR_SS.k0} ==> ={SPR_SS.O_SPR_SS.g})
-                  (SPR_SS.k0{1} = R_SPRNK_SPR.k0{2} 
-                   ==> 
-                   SPR_SS.O_SPR_SS.g{1}
-                   = 
-                   (fun k =>  
-                     if k = R_SPRNK_SPR.k0{2}
-                     then O_NK_Default.gk{2}
-                     else R_SPRNK_SPR.g{2} k)); 1,2: by smt().
-  - by call Eqv_fixone_if_dfc.
-  inline *.
-  wp; sp.
-  rnd; rnd.
-  by skip.
-wp.
-call (:   SPR_SS.k0{1} = R_SPRNK_SPR.k0{2} 
-       /\ SPR_SS.O_SPR_SS.g{1} 
-          =
-          (fun (k : key) =>
-            if k = R_SPRNK_SPR.k0{2}
-            then O_NK_Default.gk{2}
-            else R_SPRNK_SPR.g{2} k)).
-+ proc; inline *.
-  by wp; skip.
-by wp; rnd; skip.
-qed.
-
-
-local module SPR_NK_Rep (A : Adv_SPR_NK) = {
-  var x0 : input
-  var y0 : output
-  var f : input -> output
-  
-  module O_SPR_NK_Rep : Oracle_NK_t = {
-    proc get(x : input) : output = {
-      var b;
-      
-      b <@ BFOF.query(x);
-      
-      return if !b /\ x <> x0 then f x else y0;
-    }
-  }
-
-  proc main() : bool = {
-    var x' : input;
-    var y' : output;
-    
-    BFOF.init();
-
-    x0 <$ dinput;
-    y0 <$ doutput;
-
-    f <$ MUFF_In.dfun (fun _ => doutput \ (pred1 y0));    
-    
-    x' <@ A(O_SPR_NK_Rep).find(x0);
-    
-    y' <@ O_SPR_NK_Rep.get(x');
-    
-    return x' <> x0 /\ y' = y0;
-  }
-}.
-
-local lemma EqPr_SPRNK_SPRNKRep &m :
-  Pr[SPR_NK(R_SPRNK_SPR(A), O_NK_Default).main() @ &m : res]
-  =
-  Pr[SPR_NK_Rep(R_SPRNK_SPR(A)).main() @ &m : res].
-proof.
-byequiv=> //=.
-proc; inline *.
-wp.
-call (: ={R_SPRNK_SPR.k0, R_SPRNK_SPR.g} /\
-        (forall (x : input), 
-          O_NK_Default.gk{1} x 
-          = 
-          if !BFOF.f{2} x /\ x <> SPR_NK_Rep.x0{2} 
-          then SPR_NK_Rep.f{2} x 
-          else SPR_NK_Rep.y0{2})).
-+ by proc; inline *; auto => /> &1 &2 /(_ x{2}).
-rnd; rnd; wp.
-swap{1} 2 -1; swap{2} 2 -1.
-seq 1 1 : (={glob A} /\ x{1} = SPR_NK_Rep.x0{2}); 1: by rnd.
-conseq (_ : _ 
-            ==> 
-            (forall (x : input), 
-              O_NK_Default.gk{1} x 
-              = 
-              if !BFOF.f{2} x /\ x <> SPR_NK_Rep.x0{2} 
-              then SPR_NK_Rep.f{2} x 
-              else SPR_NK_Rep.y0{2})).
-+ move=> /> &2 gk fl y0 br ih k kin gL glin r.
-  by rewrite (eq_sym r); congr; rewrite !ih //= /#.
-transitivity{1} {O_NK_Default.gk <@ LR.LambdaRepro.left();}
-                (true ==> ={O_NK_Default.gk})
-                (x{1} = SPR_NK_Rep.x0{2} 
-                 ==> 
-                 (forall (x : input),
-                   O_NK_Default.gk{1} x 
-                   =
-                   if ! BFOF.f{2} x /\ x <> SPR_NK_Rep.x0{2} 
-                   then SPR_NK_Rep.f{2} x
-                   else SPR_NK_Rep.y0{2})); 1,2: by smt().
-+ inline *.
-  by wp; rnd.
-transitivity{1} {O_NK_Default.gk <@ LR.LambdaRepro.right(x);}
-                (true ==> ={O_NK_Default.gk})
-                (x{1} = SPR_NK_Rep.x0{2} 
-                 ==> 
-                 (forall (x : input),
-                   O_NK_Default.gk{1} x 
-                   =
-                   if ! BFOF.f{2} x /\ x <> SPR_NK_Rep.x0{2} 
-                   then SPR_NK_Rep.f{2} x
-                   else SPR_NK_Rep.y0{2})); 1,2: by smt().
-+ by call LR.main_theorem.
-inline *.
-wp; rnd.
-swap{2} 1 1.
-by rnd; rnd; wp; skip.
-qed.  
-
-
-local lemma EqPr_SPR_SPRNKRep &m:
-  Pr[SPR(A, O_Default).main() @ &m : res]
-  =
-  Pr[SPR_NK_Rep(R_SPRNK_SPR(A)).main() @ &m : res].
-proof. 
-by rewrite EqPr_SPR_SPRSS EqPr_SPRSS_SPRNK EqPr_SPRNK_SPRNKRep. 
-qed.
-
-local lemma SPRNKRep_Implies_BFFind &m :
-  Pr[SPR_NK_Rep(R_SPRNK_SPR(A)).main() @ &m : res] 
-  <= 
-  Pr[BF_Find(R_BFFind_SPRNK(A), BFOF).main() @ &m : res].
-proof.
-byequiv=> //=.
-proc; inline *.
-wp.
-conseq (: ={glob A} ==> ={BFOF.f, x'0} /\ SPR_NK_Rep.f{1} x'0{1} <> SPR_NK_Rep.y0{1}) => // />; 1: by smt().
-call (:   ={glob BFOF, R_SPRNK_SPR.k0, R_SPRNK_SPR.g}
-       /\ SPR_NK_Rep.y0{1} = R_BFFind_SPRNK.y0{2}
-       /\ SPR_NK_Rep.f{1} = R_BFFind_SPRNK.f{2}
-       /\ SPR_NK_Rep.x0{1} = R_BFFind_SPRNK.x0{2}).
-+ proc; inline *.
-  by wp; skip.
-rnd; rnd; wp; rnd; rnd; rnd; rnd; skip =>/> fL flin x0 x0in y0 y0in fl' flpin k kin g gin r.
-move/MUFF_In.dfun_supp: flpin => /= /(_ r).
-by rewrite supp_dexcepted /pred1 /=.
-qed.
-
-local lemma SPR_Implies_BFDistinguish &m:
-  Pr[KHFO_SPR.SPR(A, KHFO.O_Default).main() @ &m : res]
-  <=
-  `| Pr[BF_Distinguish(R_BFDistinguish_BFFind(R_BFFind_SPRNK(A)), BFOD).main(false) @ &m : res] - 
-     Pr[BF_Distinguish(R_BFDistinguish_BFFind(R_BFFind_SPRNK(A)), BFOD).main(true) @ &m : res] |.
-proof.
-apply (StdOrder.RealOrder.ler_trans Pr[BF_Find(R_BFFind_SPRNK(A), BFOF).main() @ &m : res]); last first.
-+ by rewrite (Find_Implies_Distinguish &m (R_BFFind_SPRNK(A))).
-by rewrite EqPr_SPR_SPRNKRep SPRNKRep_Implies_BFFind.
-qed.
-
-end section.
-
-end SPRBound.
-*)
-
-(*
-theory SPRBound.
-
-type key.
-type input.
-type output.
-
-clone import FinType as FinKey with
-  type t <= key.
-
-clone import FinType as FinIn with
-  type t <= input.
-
-clone import FinProdType as FinKeyIn with
-  type t1 <= key,
-  type t2 <- input,
-  
-  theory FT1 <= FinKey,
-  theory FT2 <= FinIn.
-  
-clone import FinType as FinOut with
-  type t <= output.
-
-axiom gt1_cardout : 1 < FinOut.card.
-
-op [lossless] dkey : key distr.
-op [lossless] dinput : input distr.
-
-clone import MUniFinFun as MUFF_Key with
-  type t <= key,
-  
-  theory FinT <= FinKey.
-
-clone import MUniFinFun as MUFF_In with
-  type t <= input,
-  
-  theory FinT <= FinIn.
-
-clone import MUniFinFun as MUFF_KeyIn with
-  type t <= key * input,
-  
-  theory FinT <= FinKeyIn.
-
-clone import MFinite as MF_Out with
-  type t <= output,
-  
-  theory Support <= FinOut.
-
-op doutput = MF_Out.dunifin.
-
-clone import BooleanFunctions as BF with
-  type in_t <- key * input,
-  type out_t <- output,
-  
-  theory FinIn <- FinKeyIn,
-  theory FinOut <- FinOut,
-  theory LR.MUFF <- MUFF_KeyIn,
-  theory LR.MFY <- MF_Out
-  
-  proof *.
-  realize gt1_cardout by exact: gt1_cardout.
-
-    
-op [lossless full uniform] df : (key -> input -> output) distr.
-
-lemma df_funi : is_funiform df.
-proof. by rewrite is_full_funiform 1:df_fu df_uni. qed.
-
-(*
-op df' : (key -> input -> output) distr =
-  dfun (fun (k : key) => dfun (fun (x : input) => doutput)).
-
-lemma df'_ll : is_lossless df'.
-proof. by rewrite dfun_ll => k; rewrite dfun_ll => x /=; apply dunifin_ll. qed.
-
-lemma df'_fu : is_full df'.
-proof. by rewrite dfun_fu => k /=; rewrite dfun_fu => x /=; apply dunifin_fu. qed.
-
-lemma df'_uni : is_uniform df'.
-proof. by rewrite dfun_uni => k /=; rewrite dfun_uni => x /=; apply dunifin_uni. qed.
-
-lemma df'_funi : is_funiform df'.
-proof. by rewrite is_full_funiform 1:df'_fu df'_uni. qed.
-
-lemma eq_df_df' : df = df'.
-proof. by rewrite &(eq_funi_ll) 1:df_funi 1:df_ll 1:df'_funi df'_ll. qed.
-
-lemma dmap_df'_eq (k : key) :
-  dmap df' (fun f => f k) = dfun (fun (x : input) => doutput).
-proof. 
-rewrite dfun_projE /= eq_sym -{1}(dscalar1 (dfun (fun (_ : input) => doutput))) -/df'.
-by congr; rewrite df'_ll is_losslessP 1:dfun_ll //= dunifin_ll.
-qed.
-*)
-
-(* Plan:
-   - Instantiate KHFO SPR with df
-   - Instantiate KHFO SPR with df'
-   - Prove SPR with df and df' directly equivalent
-   - Create auxiliary KHFO SPR with df', say SPR', where game computes f k immediately after sampling f/k and then initializes its oracle with this function directly (not providing k).
-   - Prove regular SPR with df' equivalent to SPR'.
-   - Create another auxiliary KHFO SPR, say SPR'', where k does not exist and f is sampled from "dfun (fun (x : input) => doutput)"
-   - Prove SPR' equivalent to SPR'' by using transitivity to (1) go from SPR' to a variant that encapsulates the sampling of f and computation of f k in the "S.map" function in DMap.ec, and (2) to go from SPR'' to a variant that directly samples f from "dmap df' (fun f => f k)" (and by lemma dmap_df'_eq above, this is equivalent to sampling f as SPR'' does).
-   - At this point, SPR'' should be (close to identical) to the SPR game used in the original proof in HashFunctionBounds.ec. So, use the proof in there and adapt it so that the proof goest through here as well.
-   - Combine everything to get the full proof for the original KHFO SPR with df.
-*)
-clone import KeyedHashFunctionsO as KHFO with
-  type key_t <- key,
-  type in_t <- input,
-  type out_t <- output,
-  
-    op df <- df
-    
-  proof *.
-  realize df_ll by exact: df_ll.
-
-clone import SPR as KHFO_SPR with
-  op din <- dinput,
-  op dkey <- dkey
-  
-  proof *.
-  realize din_ll by exact: dinput_ll.
-  realize dkey_ll by exact: dkey_ll.
-
-
-module (R_BFFind_SPR (A : Adv_SPR) : Adv_BFFind) (BFO : BFOF_t) = {
-  var f : key * input -> output
-  var k0 : key
-  var x0 : input
-  var y0 : output
-  
-  module O_R_BFFind_SPR : Oracle_t = {
-    proc get(k : key, x : input) : output = {
-      var b;
-
-      b <@ BFO.query((k, x));
-      
-      return if !b /\ (k, x) <> (k0, x0) then f (k, x) else y0;
-    }
-  }
-
-  proc find() : key * input = {
-    var x' : input;
-    
-    x0 <$ dinput;
-    y0 <$ doutput;
-
-    f <$ MUFF_KeyIn.dfun (fun _ => doutput \ (pred1 y0));
-    
-    k0 <$ dkey;
-    x'  <@ A(O_R_BFFind_SPR).find(k0, x0);
-    
-    return (k0, x');
-  }
-}.
-
-
-section.
-
-declare module A <: Adv_SPR {-KHFO.O_Default, -R_BFFind_SPR, -BFOF, -BFOD}.
-
-local op df'_prod : (key * input -> output) distr =
-  dfun (fun (kx : key * input) => doutput).
-
-local lemma df'_prod_ll : is_lossless df'_prod.
-proof. by rewrite &(dfun_ll) /= dunifin_ll. qed.
-
-local lemma df'_prod_fu : is_full df'_prod.
-proof. by rewrite &(dfun_fu) /= dunifin_fu. qed.
-
-local lemma df'_prod_uni : is_uniform df'_prod.
-proof. by rewrite &(dfun_uni) /= dunifin_uni. qed.
-
-local op df' : (key -> input -> output) distr =
-  dmap df'_prod (fun (f : key * input -> output) => 
-                  (fun (k : key) => fun (x : input) => f (k, x))).
-                  
-local lemma df'_ll : is_lossless df'.
-proof. by rewrite &(dmap_ll) /= df'_prod_ll. qed.
-
-local lemma df'_fu : is_full df'.
-proof. 
-rewrite &(dmap_fu) /= 2:df'_prod_fu /surjective.
-move=> f; exists (fun (kx : key * input) => f kx.`1 kx.`2).
-by rewrite fun_ext => k; rewrite fun_ext => x.
-qed.
-
-local lemma df'_uni : is_uniform df'.
-proof.
-rewrite &(dmap_uni) /= 2:df'_prod_uni /injective.
-by move=> f g eqfg; rewrite fun_ext => kx /#.
-qed.
-
-local lemma df'_funi : is_funiform df'.
-proof. by rewrite is_full_funiform 1:df'_fu df'_uni. qed.
-
-local lemma eq_df_df' : df = df'.
-proof. by rewrite &(eq_funi_ll) 1:df_funi 1:df_ll 1:df'_funi df'_ll. qed.
-
-
-local clone import KeyedHashFunctionsO as KHFO' with
-  type key_t <- key,
-  type in_t <- input,
-  type out_t <- output,
-  
-    op df <- df'
-    
-  proof *.
-  realize df_ll by exact: df'_ll.
-
-local clone import KHFO'.SPR as KHFO'_SPR with
-  op din <- dinput,
-  op dkey <- dkey
-  
-  proof *.
-  realize din_ll by exact: dinput_ll.
-  realize dkey_ll by exact: dkey_ll.
-
-
-local equiv Equiv_KHFO_SPR_KHFO'_SPR :
-   KHFO_SPR.SPR(A, KHFO.O_Default).main ~ KHFO'_SPR.SPR(A, KHFO'.O_Default).main : ={glob A} ==> ={res}.
-proof.
-proc; inline *.
-wp; call (: ={f}(KHFO.O_Default, KHFO'.O_Default)); 1: by proc.
-wp; rnd; wp; rnd; rnd; skip => />.
-by rewrite eq_df_df'.
-qed.
-
-(*
-local clone import DMapSampling as DMS with
-  type t1 <- key -> input -> output,
-  type t2 <- input -> output
-  
-  proof *.
-
-
-local module O_Default_NK : Oracle_t = {
-  var f : input -> output
-  
-  proc init(f_init : input -> output) = {
-    f <- f_init;
-  }
-  
-  proc get(k : key, x : input) : output = {
-    return f x;
-  }
-}.
-
-local module SPR_DMS = {
-  proc main() : bool = {
-    var f : key -> input -> output;
-    var k : key;
-    var x : input;
-    var x' : input;
-
-    f <$ df';
-    k <$ dkey;
-    O_Default_NK.init(f k);
-    x <$ dinput;
-    x' <@ A(O_Default_NK).find(k, x);
-    
-    return x <> x' /\ f k x = f k x';
-  }
-  
-  proc main_map() : bool = {
-    var f : input -> output;
-    var k : key;
-    var x : input;
-    var x' : input;
-
-    k <$ dkey;
-    f <@ S.map(df', fun f => f k);
-    O_Default_NK.init(f);
-    x <$ dinput;
-    x' <@ A(O_Default_NK).find(k, x);
-    
-    return x <> x' /\ f x = f x';
-  }
-  
-  proc main_sample() : bool = {
-    var f : input -> output;
-    var k : key;
-    var x : input;
-    var x' : input;
-
-    k <$ dkey;
-    f <@ S.sample(df', fun f => f k);
-    O_Default_NK.init(f);
-    x <$ dinput;
-    x' <@ A(O_Default_NK).find(k, x);
-
-    return x <> x' /\ f x = f x';
-  }
-}.
-
-local equiv Equiv_KHFO'_SPR_SPR_DMS_Main :
-  KHFO'_SPR.SPR(A, O_Default).main ~ SPR_DMS.main : ={glob A} ==> ={res}. 
-proof.
-proc; inline *.
-call (: O_Default.f{1} O_Default.k{1} = O_Default_NK.f{2}); 1: by proc.
-by rnd; wp; rnd; rnd; skip.
-qed.
-
-
-local module SPR_NK = {
-  proc main() : bool = {
-    var f : input -> output;
-    var x, x' : input;
-    var k : key;
-    
-    f <$ dfun (fun (x : input) => doutput);
-    O_Default_NK.init(f);
-    x <$ dinput;
-    k <$ dkey;
-    x' <@ A(O_Default_NK).find(k, x);
-
-    return x <> x' /\ f x = f x';
-  }
-}.
-
-local equiv Equiv_SPR_DMS_Main_SPR_NK :
-  SPR_DMS.main ~ SPR_NK.main : ={glob A} ==> ={res}. 
-proof.
-transitivity SPR_DMS.main_map (={glob A} ==> ={res}) (={glob A} ==> ={res}) => [/# | // | |].
-+ proc; inline *.
-  call (: ={O_Default_NK.f}); 1: by proc.
-  swap{1} 2 -1.
-  by rnd; wp; rnd; wp; rnd; skip.
-transitivity SPR_DMS.main_sample (={glob A} ==> ={res}) (={glob A} ==> ={res}) => [/# | // | |].
-+ proc; inline O_Default_NK.init.
-  call (: ={O_Default_NK.f}); 1: by proc.
-  rnd; wp => /=.
-  by symmetry; call DMS.sample; rnd; skip.
-proc; inline *.
-swap{2} 5 -4.
-wp; call (: ={O_Default_NK.f}); 1: by proc.
-wp; rnd; wp; rnd; wp; rnd; skip => /> k kin. 
-by rewrite dmap_df'_eq.
-qed.
-
-local lemma EqPr_SPR_SPR_NK &m :
-  Pr[KHFO_SPR.SPR(A, KHFO.O_Default).main() @ &m : res]
-  =
-  Pr[SPR_NK.main() @ &m : res].
-proof.
-byequiv=> //=.
-transitivity KHFO'_SPR.SPR(A, KHFO'.O_Default).main 
-             (={glob A} ==> ={res}) 
-             (={glob A} ==> ={res}) => [/# | // | |].
-+ by apply Equiv_KHFO_SPR_KHFO'_SPR.                
-transitivity SPR_DMS.main 
-             (={glob A} ==> ={res}) 
-             (={glob A} ==> ={res}) => [/# | // | |].
-+ by apply Equiv_KHFO'_SPR_SPR_DMS_Main.                
-by apply Equiv_SPR_DMS_Main_SPR_NK.
-qed.
-*)
-
-
-local clone import DMapSampling as DMS with
-  type t1 <- key -> input -> output,
-  type t2 <- key * input -> output
-  
-  proof *.
-
-local module O_Default_Uncurry : Oracle_t = {
-  var f : key * input -> output
-  
-  proc init(f_init : key * input -> output) = {
-    f <- f_init;
-  }
-  
-  proc get(k : key, x : input) : output = {
-    return f (k, x);
-  }
-}.
-
-local module SPR_DMS = {
-  proc main() : bool = {
-    var f : key -> input -> output;
-    var k : key;
-    var x : input;
-    var x' : input;
-
-    f <$ df';
-    k <$ dkey;
-    O_Default_Uncurry.init((fun (kx : key * input) => f kx.`1 kx.`2));
-    x <$ dinput;
-    x' <@ A(O_Default_Uncurry).find(k, x);
-    
-    return x' <> x /\ f k x' = f k x;
-  }
-
-  proc main_sample() : bool = {
-    var f : key * input -> output;
-    var k : key;
-    var x : input;
-    var x' : input;
-
-    f <@ S.sample(df', fun f => (fun (kx : key * input) => f kx.`1 kx.`2));
-    k <$ dkey;
-    O_Default_Uncurry.init(f);
-    x <$ dinput;
-    x' <@ A(O_Default_Uncurry).find(k, x);
-
-    return x' <> x /\ f (k, x') = f (k, x);
-  }
-
-  proc main_map() : bool = {
-    var f : key * input -> output;
-    var k : key;
-    var x : input;
-    var x' : input;
-
-    f <@ S.map(df', fun f => (fun (kx : key * input) => f kx.`1 kx.`2));
-    k <$ dkey;
-    O_Default_Uncurry.init(f);
-    x <$ dinput;
-    x' <@ A(O_Default_Uncurry).find(k, x);
-    
-    return x' <> x /\ f (k, x') = f (k, x);
-  }
-}.
-
-local equiv Equiv_KHFO'_SPR_SPR_DMS_Main :
-  KHFO'_SPR.SPR(A, O_Default).main ~ SPR_DMS.main : ={glob A} ==> ={res}. 
-proof.
-proc; inline *.
-wp; call (: forall (k : key) (x : input),
-              O_Default.f{1} k x = O_Default_Uncurry.f{2} (k, x)).
-by proc; skip => /> /#.
-by wp; rnd; wp; rnd; rnd; skip.
-qed.
-
-local module SPR_Uncurry = {
-  proc main() : bool = {
-    var f : key * input -> output;
-    var x, x' : input;
-    var k : key;
-    
-    f <$ df'_prod;
-    k <$ dkey;
-    O_Default_Uncurry.init(f);
-    x <$ dinput;
-    x' <@ A(O_Default_Uncurry).find(k, x);
-
-    return x' <> x /\ f (k, x') = f (k, x);
-  }
-}.
-
-local equiv Equiv_SPR_DMS_Main_SPR_Uncurry :
-  SPR_DMS.main ~ SPR_Uncurry.main : ={glob A} ==> ={res}. 
-proof.
-transitivity SPR_DMS.main_map (={glob A} ==> ={res}) (={glob A} ==> ={res}) => [/# | // | |].
-+ proc; inline *.
-  call (: ={O_Default_Uncurry.f}); 1: by proc.
-  swap{1} 2 -1; swap{2} 5 -4.
-  by rnd; wp; rnd; wp; rnd; skip.
-transitivity SPR_DMS.main_sample (={glob A} ==> ={res}) (={glob A} ==> ={res}) => [/# | // | |].
-+ proc; inline O_Default_Uncurry.init.
-  call (: ={O_Default_Uncurry.f}); 1: by proc.
-  rnd; wp; rnd => /=.
-  by symmetry; call DMS.sample.
-proc; inline *.
-call (: ={O_Default_Uncurry.f}); 1: by proc.
-rnd; wp; rnd; wp; rnd; wp; skip => />. 
-split => [fR fRin | _ fL] /=; 2: by rewrite df'_prod_fu.
-by rewrite dmap_comp dmap1E /(\o) /pred1; congr; rewrite fun_ext => f /#.
-qed.
-
-local lemma EqPr_SPR_SPR_Uncurry &m :
-  Pr[KHFO_SPR.SPR(A, KHFO.O_Default).main() @ &m : res]
-  =
-  Pr[SPR_Uncurry.main() @ &m : res].
-proof.
-byequiv=> //=.
-transitivity KHFO'_SPR.SPR(A, KHFO'.O_Default).main 
-             (={glob A} ==> ={res}) 
-             (={glob A} ==> ={res}) => [/# | // | |].
-+ by apply Equiv_KHFO_SPR_KHFO'_SPR.                
-transitivity SPR_DMS.main 
-             (={glob A} ==> ={res}) 
-             (={glob A} ==> ={res}) => [/# | // | |].
-+ by apply Equiv_KHFO'_SPR_SPR_DMS_Main.                
-by apply Equiv_SPR_DMS_Main_SPR_Uncurry.
-qed.
-
-
-local module R_Find_SPR_Uncurry_Rand = {
-  import var R_BFFind_SPR
-  
-  module O_R_Find_SPR_Uncurry_Rand : Oracle_t = {
-    proc get(k : key, x : input) : output = {
-      var b;
-
-      b <@ BFOF.query((k, x));
-      
-      return if !b /\ (k, x) <> (k0, x0) then f (k, x) else y0;
-    }
-  }
-
-  proc find() : bool = {
-    var x' : input;
-    var y' : output;
-    
-    BFOF.init();
-    
-    x0 <$ dinput;
-    y0 <$ doutput;
-
-    f <$ MUFF_KeyIn.dfun (fun _ => doutput \ (pred1 y0));
-    
-    k0 <$ dkey;
-    x'  <@ A(O_R_Find_SPR_Uncurry_Rand).find(k0, x0);
-    
-    y' <@ O_R_Find_SPR_Uncurry_Rand.get((k0, x'));
-    
-    return x' <> x0 /\ y' = y0;
-  }
-}.
-
-local lemma Find_SPR_Uncurry_Rand_Implies_BFFind &m :
-  Pr[R_Find_SPR_Uncurry_Rand.find() @ &m : res] 
-  <= 
-  Pr[BF_Find(R_BFFind_SPR(A), BFOF).main() @ &m : res].
-proof.
-byequiv=> //=.
-proc; inline *.
-wp.
-conseq (_: ={glob A} 
-           ==> 
-               ={BFOF.f, R_BFFind_SPR.k0, x'} 
-            /\ R_BFFind_SPR.f{1} (R_BFFind_SPR.k0, x'){1} <> R_BFFind_SPR.y0{1}) => />; 1: by smt().
-call (: ={glob BFOF, glob R_BFFind_SPR}); 1: by sim.
-do 5! rnd; skip => /> fL fLin x0L x0Lin y0L y0Lin fL' + k kin r. 
-by rewrite dfun_supp => /(_ (k, r)) /=; rewrite supp_dexcepted /pred1 /= => -[_ ->].
-qed.
-
-local lemma EqPr_SPR_Uncurry_BFFind &m :
-  Pr[SPR_Uncurry.main() @ &m: res] 
-  = 
-  Pr[R_Find_SPR_Uncurry_Rand.find() @ &m : res].
-proof.
-byequiv=> //=.
-proc; inline *.
-wp.
-swap{1} 2 3.
-swap{1} 4 -3; swap{1} 5 -3.
-swap{2} 2 -1; swap{2} 5 -3 => /=.
-seq 2 2: (   ={glob A} 
-          /\ x{1} = R_BFFind_SPR.x0{2}
-          /\ k{1} = R_BFFind_SPR.k0{2}); 1: by rnd; rnd.
-call (: forall (k : key) (x : input),
-          O_Default_Uncurry.f{1} (k, x) 
-          = 
-          if !BFOF.f{2} (k, x) /\ (k, x) <> (R_BFFind_SPR.k0, R_BFFind_SPR.x0){2} 
-          then R_BFFind_SPR.f{2} (k, x)
-          else R_BFFind_SPR.y0{2}).
-+ proc; inline *.
-  by wp; skip => /> &1 &2 /(_ k{2} x{2}).
-wp => />; 1: smt().
-conseq (: _ ==> (forall (k : key) (x : input), 
-                   f{1} (k, x) 
-                   = 
-                   if !BFOF.f{2} (k, x) /\ (k, x) <> (R_BFFind_SPR.k0, R_BFFind_SPR.x0){2}
-                   then R_BFFind_SPR.f{2} (k, x) 
-                   else R_BFFind_SPR.y0{2})).
-+ move=> /> &2 fL fR y0 fB ih r.
-  by rewrite (eq_sym r); congr; rewrite !ih /= /#.
-transitivity {1} {f <@ LR.LambdaRepro.left();}
-  (true ==> ={f}) 
-  (k{1} = R_BFFind_SPR.k0{2} /\ x{1} = R_BFFind_SPR.x0{2} 
-   ==> 
-   forall (k : key) (x : input), 
-     f{1} (k, x) 
-     = 
-     if ! BFOF.f{2} (k, x) /\ (k, x) <> (R_BFFind_SPR.k0, R_BFFind_SPR.x0){2} 
-     then  R_BFFind_SPR.f{2} (k, x) 
-     else  R_BFFind_SPR.y0{2}) => //.
-+ by move=> &1 &2 ?; exists R_BFFind_SPR.k0{2} R_BFFind_SPR.x0{2}.
-+ by inline *; wp; rnd.
-transitivity {1} {R_BFFind_SPR.f <@ LR.LambdaRepro.right(k, x);}
-  (true ==> f{1} = R_BFFind_SPR.f{2}) 
-  (k{1} = R_BFFind_SPR.k0{2} /\ x{1} = R_BFFind_SPR.x0{2} 
-   ==> 
-   forall (k : key) (x : input), 
-     R_BFFind_SPR.f{1} (k, x) 
-     = 
-     if ! BFOF.f{2} (k, x) /\ (k, x) <> (R_BFFind_SPR.k0, R_BFFind_SPR.x0){2} 
-     then R_BFFind_SPR.f{2} (k, x) 
-     else R_BFFind_SPR.y0{2}) => //.
-+ by move=> &1 &2 ?; exists R_BFFind_SPR.k0{2} R_BFFind_SPR.x0{2}.
-+ by call LR.main_theorem. 
-inline *; swap{1} 3 -1.
-by wp; rnd; rnd; rnd; wp; skip. 
-qed.
-
-lemma SPR_Implies_BFDistinguish &m:
-  Pr[KHFO_SPR.SPR(A, KHFO.O_Default).main() @ &m : res]
-  <=
-  `| Pr[BF_Distinguish(R_BFDistinguish_BFFind(R_BFFind_SPR(A)), BFOD).main(false) @ &m : res] - 
-     Pr[BF_Distinguish(R_BFDistinguish_BFFind(R_BFFind_SPR(A)), BFOD).main(true) @ &m : res] |.
-proof.
-apply (StdOrder.RealOrder.ler_trans Pr[BF_Find(R_BFFind_SPR(A), BFOF).main() @ &m : res]); last first.
-+ by rewrite (Find_Implies_Distinguish &m (R_BFFind_SPR(A))).
-by rewrite EqPr_SPR_SPR_Uncurry EqPr_SPR_Uncurry_BFFind Find_SPR_Uncurry_Rand_Implies_BFFind.
-qed.
-
-end section.
-
-end SPRBound.
-*)
-
-(* 
-  Try and use Reprogramming.ec theory to do this prove.
-*)
+(** Bound for TCR **)
 theory TCRBound.
 
 op [lossless full uniform] dkey : key distr.
@@ -1766,41 +460,6 @@ section.
 
 declare module A <: Adv_TCR {-KHFO.O_Default, -BFOF, -BFOD, -R_BFFind_TCR, -Counting_O}.
 
-declare axiom A_pick_ll (O <: Oracle_t{-A}):
-  islossless O.get => islossless A(O).pick.
-
-declare axiom A_find_ll (O <: Oracle_t{-A}):
-  islossless O.get => islossless A(O).find.
-
-
-local module TCR_DFC = {
-  module O_TCR_DFC : Oraclei_t = {
-    var g : key -> input -> output
-    
-    proc init() : unit ={
-      g <$ dfc;
-    }
-    
-    proc get(k : key, x : input) : output = {
-      return g k x;
-    }
-  }
-  
-  proc main = KHFO_TCR.TCR(A, O_TCR_DFC).main  
-}.
-
-local lemma EqPr_TCR_TCR_DFC &m :
-  Pr[KHFO_TCR.TCR(A, O_Default).main() @ &m : res]
-  =
-  Pr[TCR_DFC.main() @ &m : res]. 
-proof.
-byequiv=> //.
-proc.
-seq 1 1: (={glob A} /\ O_Default.f{1} = TCR_DFC.O_TCR_DFC.g{2}); 2: by sim.
-inline *.
-by rnd; skip; rewrite eq_df_dfc.
-qed.
-
 local module TCR_NoRep = {
   var k0 : key
   var g : key -> input -> output
@@ -1828,9 +487,8 @@ local module TCR_NoRep = {
   }  
 }.
 
-
-local lemma EqPr_TCR_DFC_TCR_NoRep &m :
-  Pr[TCR_DFC.main() @ &m : res] 
+local lemma EqPr_TCR_TCR_NoRep &m :
+  Pr[KHFO_TCR.TCR(A, KHFO.O_Default).main() @ &m : res] 
   =
   Pr[TCR_NoRep.main() @ &m : res].
 proof.
@@ -1838,16 +496,11 @@ byequiv=> //.
 proc; inline *.
 swap{1} 3 - 2.
 seq 2 2: (   ={glob A} 
-          /\ ={g}(TCR_DFC.O_TCR_DFC, TCR_NoRep)
+          /\ O_Default.f{1} = TCR_NoRep.g{2}
           /\ k{1} = TCR_NoRep.k0{2}).
-+ by rnd; rnd.
-wp.
-call (: ={g}(TCR_DFC.O_TCR_DFC, TCR_NoRep)).
-+ by proc.
-wp.
-call (: ={g}(TCR_DFC.O_TCR_DFC, TCR_NoRep)).
-+ by proc.
-by skip.
++ rnd; rnd; skip => />.
+  by rewrite eq_df_dfc.
+by sim.
 qed.
 
 
@@ -1898,107 +551,10 @@ local module TCR_Rep = {
 local clone import DFun as DF with
   type in_t <- key,
   type out_t <- input -> output,
-    op dout <- dfcs,
     
   theory FT_In <- FinKey
   
   proof *.
-  realize dout_ll by exact: dfcs_ll.
-(*
-local module TCR_NoRep_Fmap = {
-  var k0 : key
-  var gk : input -> output
-  var g : (key, input -> output) fmap
-    
-  module O_TCR_NoRep : Oracle_t = {
-    proc get(k : key, x : input) : output = {
-      return (oget g.[k]) x;
-    }
-  }
-    
-  proc main() : bool = {
-    var x, x' : input;
-    var y, y' : output;
-    var w : key list;
-    var k : key;
-    var f : input -> output;
-    
-    k0 <$ dkey;
-    gk <$ dfcs;
-    
-    w <- FinKey.enum;
-    g <- empty;
-    while (w <> []){
-      k <- head witness w;
-      f <$ dfcs;
-      g.[k] <- f;
-      w <- behead w;
-    }
-    
-    x <@ A(O_TCR_NoRep).pick();
-    y <@ O_TCR_NoRep.get(k0, x);
-    
-    x' <@ A(O_TCR_NoRep).find(k0);
-    y' <@ O_TCR_NoRep.get(k0, x');
-    
-    return x' <> x /\ y' = y;
-  }  
-}.
-
-local module TCR_Rep_Fmap = {
-  var k0 : key
-  var gk : input -> output
-  var g : (key, input -> output) fmap
-    
-  module O_TCR_Rep_Pick : Oracle_t = {
-    proc get(k : key, x : input) : output = {
-      return (oget g.[k]) x;
-    }
-  }
-  
-  module O_TCR_Rep_Find : Oracle_t = {
-    proc get(k : key, x : input) : output = {
-      var y : output;
-      
-      if (k = k0) {
-        y <- gk x;
-      } else {
-        y <- (oget g.[k] x);
-      }
-      
-      return y;
-    }
-  }
-  
-  proc main() : bool = {
-    var x, x' : input;
-    var y, y' : output;
-    var w : key list;
-    var k : key;
-    var f : input -> output;
-    
-    k0 <$ dkey;
-    gk <$ dfcs;
-    
-    w <- FinKey.enum;
-    g <- empty;
-    while (w <> []){
-      k <- head witness w;
-      f <$ dfcs;
-      g.[k] <- f;
-      w <- behead w;
-    }
-    
-    x <@ A(O_TCR_Rep_Pick).pick();
-    y <@ O_TCR_Rep_Find.get(k0, x);
-    
-    x' <@ A(O_TCR_Rep_Find).find(k0);
-    y' <@ O_TCR_Rep_Find.get(k0, x');
-    
-    return x' <> x /\ y' = y;
-  }  
-}.
-*)
 
 local clone import Reprogramming as Repro with
   type in_t <- key,
@@ -2021,7 +577,7 @@ local module TCR_NoRep_ERO = {
       var f : input -> output;
       var y : output;
       
-      f <@ Wrapped_Oracle(ERO).o(k);
+      f <@ O_Programmable(ERO).o(k);
       
       return f x;
     }
@@ -2033,7 +589,7 @@ local module TCR_NoRep_ERO = {
     var k : key;
     
     ERO.init();
-    Wrapped_Oracle(ERO).init();
+    O_Programmable(ERO).init();
     
     x <@ A(O_TCR_NoRep).pick();
     
@@ -2055,7 +611,7 @@ local module TCR_Rep_ERO = {
       var f : input -> output;
       var y : output;
       
-      f <@ Wrapped_Oracle(ERO).o(k);
+      f <@ O_Programmable(ERO).o(k);
       
       return f x;
     }
@@ -2068,14 +624,14 @@ local module TCR_Rep_ERO = {
     var gk : input -> output;
     
     ERO.init();
-    Wrapped_Oracle(ERO).init();
+    O_Programmable(ERO).init();
     
     x <@ A(O_TCR_Rep).pick();
     
     k <$ dkey;
     gk <$ dfcs;
     
-    Wrapped_Oracle(ERO).set(k, gk);
+    O_Programmable(ERO).set(k, gk);
     
     y <@ O_TCR_Rep.get(k, x);
     
@@ -2102,26 +658,30 @@ do 2! congr; last congr.
              /\ TCR_NoRep.g{1} = (fun (k' : key) => oget ERO.m{2}.[k'])).
   - rnd.
     conseq (: true ==> TCR_NoRep.g{1} = (fun (k' : key) => oget ERO.m{2}.[k'])) => //.
-    transitivity{1} {TCR_NoRep.g <@ Direct.sample();}
+    transitivity{1} {TCR_NoRep.g <@ Direct_Fun.sample(kdfcs);}
                     (true ==> ={TCR_NoRep.g})
                     (true ==> TCR_NoRep.g{1} = (fun (k' : key) => oget ERO.m{2}.[k'])) => //.
-    * by inline *; wp; rnd.
-    transitivity{2} {ERO.m <@ Loop_Fmap_Head.sample();}
+    * by inline *; wp; rnd; wp.
+    transitivity{2} {ERO.m <@ Loop_Fmap.sample(kdfcs, FinKey.enum);}
                     (true ==> TCR_NoRep.g{1} = (fun (k' : key) => oget ERO.m{2}.[k']))
                     (true ==> ={ERO.m}) => //.
     * symmetry.
-      call Eqv_Loop_Fmap_Head_Direct_Map.
+      call (Eqv_Loop_Fmap_Direct_Fun kdfcs).
       by skip.
-    by inline *; swap{1} 1 1; sim.
+    inline *.
+    wp; sp. 
+    while (d{1} = kdfcs /\ m{1} = ERO.m{2} /\ xs{1} = w{2}).
+    * by wp; rnd; wp; skip.
+    by skip.
   inline *.
   wp; sp => /=.
   call (:   TCR_NoRep.g{1} = (fun (k' : key) => oget ERO.m{2}.[k'])
-         /\ Wrapped_Oracle.prog_list{2} = []).
+         /\ O_Programmable.prog_list{2} = []).
   - proc; inline *.
     by wp; skip.
   wp.
   call (:    TCR_NoRep.g{1} = (fun (k' : key) => oget ERO.m{2}.[k'])
-          /\ Wrapped_Oracle.prog_list{2} = []).
+          /\ O_Programmable.prog_list{2} = []).
   - proc; inline *.
     by wp; skip.
   by skip.
@@ -2134,35 +694,37 @@ seq 3 3 : (   ={glob A}
            /\ TCR_Rep.g{1} = (fun (k' : key) => oget ERO.m{2}.[k'])).
 + rnd; rnd.
   conseq (: true ==> TCR_Rep.g{1} = (fun (k' : key) => oget ERO.m{2}.[k'])) => //.
-  transitivity{1} {TCR_Rep.g <@ Direct.sample();}
+  transitivity{1} {TCR_Rep.g <@ Direct_Fun.sample(kdfcs);}
                   (true ==> ={TCR_Rep.g})
                   (true ==> TCR_Rep.g{1} = (fun (k' : key) => oget ERO.m{2}.[k'])) => //.
-  - by inline *; wp; rnd.
-  transitivity{2} {ERO.m <@ Loop_Fmap_Head.sample();}
+  - by inline *; wp; rnd; wp.
+  transitivity{2} {ERO.m <@ Loop_Fmap.sample(kdfcs, FinKey.enum);}
                   (true ==> TCR_Rep.g{1} = (fun (k' : key) => oget ERO.m{2}.[k']))
                   (true ==> ={ERO.m}) => //.
   - symmetry.
-    call Eqv_Loop_Fmap_Head_Direct_Map.
+    call (Eqv_Loop_Fmap_Direct_Fun kdfcs).
     by skip.
-  by inline *; swap{1} 1 1; sim.
+  inline *.
+  wp; sp. 
+  while (d{1} = kdfcs /\ m{1} = ERO.m{2} /\ xs{1} = w{2}).
+  - by wp; rnd; wp; skip.
+  by skip.
 inline *.
 wp; sp => /=.
 call (:   TCR_Rep.g{1} = (fun (k' : key) => oget ERO.m{2}.[k'])
-       /\ Wrapped_Oracle.prog_list{2} = [(TCR_Rep.k0{1}, TCR_Rep.gk{1})]).
+       /\ O_Programmable.prog_list{2} = [(TCR_Rep.k0{1}, TCR_Rep.gk{1})]).
 + proc; inline *.
   wp; skip => /> &1 &2 neqk.
   by rewrite assoc_cons neqk assoc_nil.
 wp => /=.
 call (:   TCR_Rep.g{1} = (fun (k' : key) => oget ERO.m{2}.[k'])
-       /\ Wrapped_Oracle.prog_list{2} = []).
+       /\ O_Programmable.prog_list{2} = []).
 + proc; inline *.
   by wp; skip.
 by skip.
 qed.
 
-local module (R_Repro_TCR : DistA) (O : POracle, RepO : RepO_t) = {  
-  var k0 : key
-  
+local module (R_Repro_TCR : Adv_INDRepro) (O : POracle, OR : Oracler_t) = {  
   module O_R_Repro_TCR : Oracle_t = {
     proc get(k : key, x : input) = {
       var f : input -> output;
@@ -2175,12 +737,13 @@ local module (R_Repro_TCR : DistA) (O : POracle, RepO : RepO_t) = {
   }
   
   proc distinguish() : bool = {
+    var k0 : key;
     var x, x' : input;
     var y, y' : output;
     
     x <@ A(O_R_Repro_TCR).pick();
     
-    k0 <@ RepO.repro(dkey);
+    k0 <@ OR.repro(dkey);
     y <@ O_R_Repro_TCR.get(k0, x);
     
     x' <@ A(O_R_Repro_TCR).find(k0);
@@ -2194,16 +757,16 @@ local lemma EqPr_TCR_ERO_ReproGame &m :
   `| Pr[TCR_NoRep_ERO.main() @ &m : res] - 
      Pr[TCR_Rep_ERO.main() @ &m : res] |
    =
-  `| Pr[ReproGame(ERO, R_Repro_TCR).main(false) @ &m : res] - 
-     Pr[ReproGame(ERO, R_Repro_TCR).main(true) @ &m : res] |.
+  `| Pr[IND_Repro(ERO, R_Repro_TCR).main(false) @ &m : res] - 
+     Pr[IND_Repro(ERO, R_Repro_TCR).main(true) @ &m : res] |.
 proof.
 do 2! congr; last congr.
 + byequiv => //.
   proc.
-  seq 2 2 : (   ={glob A, glob Wrapped_Oracle, ERO.m}
+  seq 2 2 : (   ={glob A, glob O_Programmable, ERO.m}
              /\ b{2} = false
-             /\ Wrapped_Oracle.prog_list{2} = []
-             /\ Wrapped_Oracle.ch{2} = 0).
+             /\ O_Programmable.prog_list{2} = []
+             /\ O_Programmable.ch{2} = 0).
   - inline *.
     wp => /=.
     while (={w, ERO.m}).
@@ -2211,7 +774,7 @@ do 2! congr; last congr.
     by wp; skip.
   inline *.
   wp; sp => /=.
-  call (: ={glob Wrapped_Oracle, ERO.m}).
+  call (: ={glob O_Programmable, ERO.m}).
   - proc; inline *.
     by wp; skip.
   wp.
@@ -2220,16 +783,16 @@ do 2! congr; last congr.
     rnd; wp.
     by call (: true).
   rnd; wp => /=.
-  call (: ={glob Wrapped_Oracle, ERO.m}).
+  call (: ={glob O_Programmable, ERO.m}).
   - proc; inline *.
     by wp; skip.
   by skip.
 byequiv => //.
 proc.
-seq 2 2 : (   ={glob A, glob Wrapped_Oracle, ERO.m}
+seq 2 2 : (   ={glob A, glob O_Programmable, ERO.m}
            /\ b{2} = true
-           /\ Wrapped_Oracle.prog_list{2} = []
-           /\ Wrapped_Oracle.ch{2} = 0).
+           /\ O_Programmable.prog_list{2} = []
+           /\ O_Programmable.ch{2} = 0).
 + inline *.
   wp => /=.
   while (={w, ERO.m}).
@@ -2237,7 +800,7 @@ seq 2 2 : (   ={glob A, glob Wrapped_Oracle, ERO.m}
   by wp; skip.
 inline *.
 wp; sp => /=.
-call (: ={glob Wrapped_Oracle, ERO.m}).
+call (: ={glob O_Programmable, ERO.m}).
 + proc; inline *.
   by wp; skip.
 wp.
@@ -2246,7 +809,7 @@ rcondt{2} 6.
   rnd; wp.
   by call (: true).
 wp; rnd; rnd; wp.
-call (: ={glob Wrapped_Oracle, ERO.m}).
+call (: ={glob O_Programmable, ERO.m}).
 + proc; inline *.
   by wp; skip.
 by skip.
@@ -2399,10 +962,10 @@ local lemma TCR_Implies_BFDistinguish_A &m:
   `| Pr[BF_Distinguish(R_BFDistinguish_BFFind(R_BFFind_TCR(A)), BFOD).main(false) @ &m : res] - 
      Pr[BF_Distinguish(R_BFDistinguish_BFFind(R_BFFind_TCR(A)), BFOD).main(true) @ &m : res] |
   +
-  `| Pr[ReproGame(ERO, R_Repro_TCR).main(false) @ &m : res] - 
-     Pr[ReproGame(ERO, R_Repro_TCR).main(true) @ &m : res] |.  
+  `| Pr[IND_Repro(ERO, R_Repro_TCR).main(false) @ &m : res] - 
+     Pr[IND_Repro(ERO, R_Repro_TCR).main(true) @ &m : res] |.  
 proof.
-rewrite EqPr_TCR_TCR_DFC EqPr_TCR_DFC_TCR_NoRep.
+rewrite EqPr_TCR_TCR_NoRep.
 rewrite -StdOrder.RealOrder.ger0_norm 1:Pr[mu_ge0] //-{1}StdOrder.RealOrder.Domain.subr0.
 rewrite -(StdOrder.RealOrder.Domain.subrr Pr[TCR_Rep.main() @ &m : res]).
 rewrite StdOrder.RealOrder.Domain.opprD StdOrder.RealOrder.Domain.addrA /=.
@@ -2433,12 +996,11 @@ declare axiom A_Pick_queries (O <: Oracle_t{-A}) (n : int):
 declare axiom A_Find_queries (O <: Oracle_t{-A}) (n : int):
   hoare[A(Counting_O(O)).find : Counting_O.ctr = n ==> Counting_O.ctr <= n + qF].
 
-local module (R_Repro_TCR_C : DistA) (O : POracle, RepO : RepO_t) = {  
-  import var R_Repro_TCR
-  
-  module O_R_Repro_TCR_C = Counting_O(R_Repro_TCR(O, RepO).O_R_Repro_TCR) 
+local module (R_Repro_TCR_C : Adv_INDRepro) (O : POracle, OR : Oracler_t) = {  
+  module O_R_Repro_TCR_C = Counting_O(R_Repro_TCR(O, OR).O_R_Repro_TCR) 
   
   proc distinguish() : bool = {
+    var k0 : key;
     var x, x' : input;
     var y, y' : output;
     
@@ -2446,7 +1008,7 @@ local module (R_Repro_TCR_C : DistA) (O : POracle, RepO : RepO_t) = {
     
     x <@ A(O_R_Repro_TCR_C).pick();
     
-    k0 <@ RepO.repro(dkey);
+    k0 <@ OR.repro(dkey);
     y <@ O_R_Repro_TCR_C.get(k0, x);
     
     x' <@ A(O_R_Repro_TCR_C).find(k0);
@@ -2457,20 +1019,20 @@ local module (R_Repro_TCR_C : DistA) (O : POracle, RepO : RepO_t) = {
 }.
 
 local hoare R_Repro_TCR_C_queries :
-  R_Repro_TCR_C(Wrapped_Oracle(ERO), RepO(Wrapped_Oracle(ERO))).distinguish :
-    Wrapped_Oracle.ch = 0 /\ RepO.ctr = 0 /\ RepO.se 
+  R_Repro_TCR_C(O_Programmable(ERO), O_Reprogrammer(O_Programmable(ERO))).distinguish :
+    O_Programmable.ch = 0 /\ O_Reprogrammer.ctr = 0 /\ O_Reprogrammer.se 
     ==>
-    Wrapped_Oracle.ch <= q + 2 /\ RepO.ctr <= 1 /\ RepO.se.
+    O_Programmable.ch <= q + 2 /\ O_Reprogrammer.ctr <= 1 /\ O_Reprogrammer.se.
 proof.
 proc.
 sp.
 inline 5; inline 8; inline 10; inline 11.
 wp => /=.
-seq 2 : (   Counting_O.ctr = Wrapped_Oracle.ch
-         /\ Wrapped_Oracle.ch <= qP 
-         /\ RepO.ctr = 1 
-         /\ RepO.se).
-+ call (: arg = dkey /\ RepO.ctr = 0 /\ RepO.se ==> RepO.ctr = 1 /\ RepO.se).
+seq 2 : (   Counting_O.ctr = O_Programmable.ch
+         /\ O_Programmable.ch <= qP 
+         /\ O_Reprogrammer.ctr = 1 
+         /\ O_Reprogrammer.se).
++ call (: arg = dkey /\ O_Reprogrammer.ctr = 0 /\ O_Reprogrammer.se ==> O_Reprogrammer.ctr = 1 /\ O_Reprogrammer.se).
   - proc; inline *.
     sp.
     conseq (: _ ==> true) => // /> ? _.
@@ -2481,38 +1043,38 @@ seq 2 : (   Counting_O.ctr = Wrapped_Oracle.ch
     by rewrite dkey_fu.
   conseq (: _ 
             ==> 
-               Counting_O.ctr = Wrapped_Oracle.ch 
-            /\ Wrapped_Oracle.ch <= qP) => //.
+               Counting_O.ctr = O_Programmable.ch 
+            /\ O_Programmable.ch <= qP) => //.
   call (:    Counting_O.ctr = 0 
-          /\ Wrapped_Oracle.ch = 0
+          /\ O_Programmable.ch = 0
           ==>
-             Counting_O.ctr = Wrapped_Oracle.ch 
+             Counting_O.ctr = O_Programmable.ch 
           /\ Counting_O.ctr <= qP) => //.
-  conseq (: Counting_O.ctr = Wrapped_Oracle.ch ==> Counting_O.ctr = Wrapped_Oracle.ch)
-         (A_Pick_queries (<: R_Repro_TCR(Wrapped_Oracle(ERO), RepO(Wrapped_Oracle(ERO))).O_R_Repro_TCR) 0) => //. 
-  proc (Counting_O.ctr = Wrapped_Oracle.ch) => //.
+  conseq (: Counting_O.ctr = O_Programmable.ch ==> Counting_O.ctr = O_Programmable.ch)
+         (A_Pick_queries (<: R_Repro_TCR(O_Programmable(ERO), O_Reprogrammer(O_Programmable(ERO))).O_R_Repro_TCR) 0) => //. 
+  proc (Counting_O.ctr = O_Programmable.ch) => //.
   proc; inline *.
   by wp; skip.
-seq 1 : (   Counting_O.ctr = Wrapped_Oracle.ch
-         /\ Wrapped_Oracle.ch <= qP + 1 
-         /\ RepO.ctr = 1 
-         /\ RepO.se).
+seq 1 : (   Counting_O.ctr = O_Programmable.ch
+         /\ O_Programmable.ch <= qP + 1 
+         /\ O_Reprogrammer.ctr = 1 
+         /\ O_Reprogrammer.se).
 + inline *.
   by wp; skip => /> /#.
-call (:    Counting_O.ctr = Wrapped_Oracle.ch 
-        /\ Wrapped_Oracle.ch <= qP + 1 
-        /\ RepO.ctr = 1 
-        /\ RepO.se
+call (:    Counting_O.ctr = O_Programmable.ch 
+        /\ O_Programmable.ch <= qP + 1 
+        /\ O_Reprogrammer.ctr = 1 
+        /\ O_Reprogrammer.se
         ==>
-        Counting_O.ctr = Wrapped_Oracle.ch 
-        /\ Wrapped_Oracle.ch <= qP + 1 + qF 
-        /\ RepO.ctr = 1 
-        /\ RepO.se).
-+ conseq (: Counting_O.ctr = Wrapped_Oracle.ch ==> Counting_O.ctr = Wrapped_Oracle.ch)
+        Counting_O.ctr = O_Programmable.ch 
+        /\ O_Programmable.ch <= qP + 1 + qF 
+        /\ O_Reprogrammer.ctr = 1 
+        /\ O_Reprogrammer.se).
++ conseq (: Counting_O.ctr = O_Programmable.ch ==> Counting_O.ctr = O_Programmable.ch)
          (: Counting_O.ctr <= qP + 1 ==> Counting_O.ctr <= qP + 1 + qF) => //.
   - exists* Counting_O.ctr; elim* => ctr.
-    conseq (A_Find_queries (<: R_Repro_TCR(Wrapped_Oracle(ERO), RepO(Wrapped_Oracle(ERO))).O_R_Repro_TCR) ctr) => //; 1: by smt().
-  proc (Counting_O.ctr = Wrapped_Oracle.ch) => //.
+    conseq (A_Find_queries (<: R_Repro_TCR(O_Programmable(ERO), O_Reprogrammer(O_Programmable(ERO))).O_R_Repro_TCR) ctr) => //; 1: by smt().
+  proc (Counting_O.ctr = O_Programmable.ch) => //.
   proc; inline *.
   by wp.
 by skip => /> /#.
@@ -2528,972 +1090,52 @@ lemma TCR_Implies_BFDistinguish &m:
 proof.
 move: (TCR_Implies_BFDistinguish_A &m).
 have -> :
-  `| Pr[ReproGame(ERO, R_Repro_TCR).main(false) @ &m : res] -
-     Pr[ReproGame(ERO, R_Repro_TCR).main(true) @ &m : res] |
+  `| Pr[IND_Repro(ERO, R_Repro_TCR).main(false) @ &m : res] -
+     Pr[IND_Repro(ERO, R_Repro_TCR).main(true) @ &m : res] |
   =
-  `| Pr[ReproGame(ERO, R_Repro_TCR_C).main(false) @ &m : res] -
-     Pr[ReproGame(ERO, R_Repro_TCR_C).main(true) @ &m : res] |.
+  `| Pr[IND_Repro(ERO, R_Repro_TCR_C).main(false) @ &m : res] -
+     Pr[IND_Repro(ERO, R_Repro_TCR_C).main(true) @ &m : res] |.
 + do 2! congr; last congr.
   - byequiv=> //. 
     proc. 
-    seq 3 3 : (={glob A, glob ERO, glob Wrapped_Oracle, glob RepO} /\ !RepO.b{1}).
+    seq 3 3 : (={glob A, glob ERO, glob O_Programmable, glob O_Reprogrammer} /\ !O_Reprogrammer.b{1}).
     * inline{1} 3; inline{2} 3.
       wp.
-      conseq (: _ ==> ={glob ERO, glob Wrapped_Oracle}) => //.
+      conseq (: _ ==> ={glob ERO, glob O_Programmable}) => //.
       by sim.
     inline *.
     rcondf{1} 6; 1: by auto; call (: true) => //.
     rcondf{2} 7; 1: by auto; call (: true) => //; auto. 
     wp.
-    call (: ={glob ERO, glob Wrapped_Oracle, glob RepO}).
+    call (: ={glob ERO, glob O_Programmable, glob O_Reprogrammer}).
     * by proc; inline *; wp.
     wp; rnd; wp.
-    call (: ={glob ERO, glob Wrapped_Oracle, glob RepO}). 
+    call (: ={glob ERO, glob O_Programmable, glob O_Reprogrammer}). 
     * by proc; inline *; wp.
     by wp.
   byequiv=> //. 
   proc. 
-  seq 3 3 : (={glob A, glob ERO, glob Wrapped_Oracle, glob RepO} /\ RepO.b{1}).
+  seq 3 3 : (={glob A, glob ERO, glob O_Programmable, glob O_Reprogrammer} /\ O_Reprogrammer.b{1}).
   - inline{1} 3; inline{2} 3.
     wp.
-    conseq (: _ ==> ={glob ERO, glob Wrapped_Oracle}) => //.
+    conseq (: _ ==> ={glob ERO, glob O_Programmable}) => //.
     by sim.
   inline *.
   rcondt{1} 6; 1: by auto; call (: true) => //.
   rcondt{2} 7; 1: by auto; call (: true) => //; auto. 
   wp.
-  call (: ={glob ERO, glob Wrapped_Oracle, glob RepO}).
+  call (: ={glob ERO, glob O_Programmable, glob O_Reprogrammer}).
   - by proc; inline *; wp.
   wp; rnd; wp; rnd; wp.
-  call (: ={glob ERO, glob Wrapped_Oracle, glob RepO}). 
+  call (: ={glob ERO, glob O_Programmable, glob O_Reprogrammer}). 
   - by proc; inline *; wp.
   by wp.
 pose BFAdv := `| _ - _ |%Real; pose ReproAdv := `| _ - _ |%Real; move => tib.
 apply (StdOrder.RealOrder.ler_trans (BFAdv + ReproAdv)) => //.
 apply StdOrder.RealOrder.ler_add => //.
-by apply (rom_reprogramming R_Repro_TCR_C 1 _ (q + 2) _ &m R_Repro_TCR_C_queries) => //; smt(ge0_q).
+by apply (Bound_IND_Repro R_Repro_TCR_C 1 _ (q + 2) _ &m R_Repro_TCR_C_queries) => //; smt(ge0_q).
 qed. 
 
 end section.
 
 end TCRBound.
-
-(*
-section.
-
-declare module A <: Adv_TCR {-KHFO.O_Default, -BFOF, -BFOD, -R_BFFind_TCR, -Counting_O}.
-
-declare axiom A_pick_ll (O <: Oracle_t{-A}):
-  islossless O.get => islossless A(O).pick.
-
-declare axiom A_find_ll (O <: Oracle_t{-A}):
-  islossless O.get => islossless A(O).find.
-
-local module TCR_SS = {
-  var k0 : key
-  
-  module O_TCR_SS : Oracle_t = {  
-    var g : key -> input -> output
-    
-    proc init() : unit = {
-      var gk : input -> output;
-      
-      gk <$ dfcs;
-      
-      g <$ dfun kdfcs.[k0 <- dunit gk];
-    }
-    
-    proc get(k : key, x : input) = {
-      return g k x;
-    }
-  }
-  
-  proc main() : bool = {
-    var x, x' : input;
-    var y, y' : output;
-    
-    k0 <$ dkey;
-    
-    O_TCR_SS.init();
-    
-    x <@ A(O_TCR_SS).pick();
-    y <@ O_TCR_SS.get(k0, x);
-    
-    x' <@ A(O_TCR_SS).find(k0);
-    y' <@ O_TCR_SS.get(k0, x');
-    
-    return x' <> x /\ y' = y;
-  }
-}.
-
-local lemma EqPr_TCR_TCRSS &m:
-  Pr[TCR(A, O_Default).main() @ &m : res]
-  =
-  Pr[TCR_SS.main() @ &m : res].
-proof.
-byequiv => //=.
-proc; inline *.
-swap{1} 3 -2.
-seq 1 1: (={glob A} /\ k{1} = TCR_SS.k0{2}); 1: by rnd.
-wp.
-conseq (: _ ==>    ={x, x', y} 
-                /\ k{1} = TCR_SS.k0{2} 
-                /\ O_Default.f{1} = TCR_SS.O_TCR_SS.g{2}); 1: by smt().
-call (: O_Default.f{1} = TCR_SS.O_TCR_SS.g{2}); 1: by proc.
-wp; call (: O_Default.f{1} = TCR_SS.O_TCR_SS.g{2}); 1: by proc.
-conseq (: _ ==> O_Default.f{1} = TCR_SS.O_TCR_SS.g{2}) => //.
-transitivity{1} {O_Default.f <$ dfc;}
-                (true ==> ={O_Default.f})
-                (true ==>  O_Default.f{1} = TCR_SS.O_TCR_SS.g{2}) => //.
-+ by rnd; skip => />; rewrite eq_df_dfc.
-rnd: *0 *0.       
-wp; skip => /> &2.
-split => [g gin | eqmug f fin]. 
-+ rewrite dmap_id; congr.
-  rewrite /dfc /kdfcs /dfcs (MUFF_Key.dfunE_dlet_fix1 _ (TCR_SS.k0{2})) /=.
-  by congr; rewrite fun_ext => f; rewrite dmap_id.
-rewrite supp_dlet /=; exists (f TCR_SS.k0{2}).
-split; 1: by rewrite dfun_fu /= 1:dunifin_fu dmap_id //= dfun_fu.
-rewrite dmap_id dfun_supp => k @/(_.[_<-_]). 
-case (TCR_SS.k0{2} = k) => [-> | ?]; 1: by rewrite supp_dunit.
-by rewrite dmap_id dfun_supp in fin => /#.
-qed.
-
-
-local module TCR_SSR = {
-  var k0 : key
-  var ks : key list
-  var gk : input -> output
-  var g : key -> input -> output
-  
-  module O_TCR_SSR_Pick : Oracle_t = {  
-    proc get(k : key, x : input) = {
-      var y : output;
-      
-      ks <- rcons ks k;
-      
-      if (k = k0) {
-        y <- gk x;
-      } else {
-        y <- g k x;
-      } 
-      
-      return y;
-    }
-  }
-
- module O_TCR_SSR_Find : Oracle_t = {  
-    proc get(k : key, x : input) = {
-      var y : output;
-      
-      if (k = k0) {
-        y <- gk x;
-      } else {
-        y <- g k x;
-      } 
-      
-      return y;
-    }
-  }
-  
-  proc main() : bool = {
-    var x, x' : input;
-    var y, y' : output;
-    
-    k0 <$ dkey;
-    
-    ks <- [];
-    
-    gk <$ dfcs;  
-    g <$ dfc;
-    
-    x <@ A(O_TCR_SSR_Pick).pick();
-    y <@ O_TCR_SSR_Find.get(k0, x);
-    
-    x' <@ A(O_TCR_SSR_Find).find(k0);
-    y' <@ O_TCR_SSR_Find.get(k0, x');
-    
-    return x' <> x /\ y' = y;
-  }
-}.
-
-local lemma EqPr_TCRSS_TCRSSR &m:
-  Pr[TCR_SS.main() @ &m : res]
-  =
-  Pr[TCR_SSR.main() @ &m : res].
-proof.
-byequiv=> //=.
-proc; inline *.
-seq 3 4 : (   ={glob A} 
-           /\ ={k0}(TCR_SS, TCR_SSR)
-           /\ TCR_SS.O_TCR_SS.g{1} 
-              = 
-              (fun (k : key) => 
-                if k = TCR_SSR.k0{2}
-                then TCR_SSR.gk{2}
-                else TCR_SSR.g{2} k)).
-+ seq 1 1 : (={glob A} /\ ={k0}(TCR_SS, TCR_SSR)); 1: by rnd.
-  sp.
-  conseq (: _ ==> TCR_SS.O_TCR_SS.g{1} 
-                  =
-                  fun (k : key) =>
-                    if k = TCR_SSR.k0{2} 
-                    then TCR_SSR.gk{2}
-                    else TCR_SSR.g{2} k) => //.
-  transitivity{1} {TCR_SS.O_TCR_SS.g <@ EquivSamplings.fixone_dfc(TCR_SS.k0);}
-                  (={TCR_SS.k0} ==> ={TCR_SS.O_TCR_SS.g})
-                  (TCR_SS.k0{1} = TCR_SSR.k0{2} 
-                   ==> 
-                   TCR_SS.O_TCR_SS.g{1}
-                   = 
-                   (fun k =>  
-                     if k = TCR_SSR.k0{2}
-                     then TCR_SSR.gk{2}
-                     else TCR_SSR.g{2} k)); 1,2: by smt().
-  - inline *.
-    wp; sp.
-    rnd; rnd.
-    by skip.
-  transitivity{1} {TCR_SS.O_TCR_SS.g <@ EquivSamplings.if_dfc(TCR_SS.k0);}
-                  (={TCR_SS.k0} ==> ={TCR_SS.O_TCR_SS.g})
-                  (TCR_SS.k0{1} = TCR_SSR.k0{2} 
-                   ==> 
-                   TCR_SS.O_TCR_SS.g{1}
-                   = 
-                   (fun k =>  
-                     if k = TCR_SSR.k0{2}
-                     then TCR_SSR.gk{2}
-                     else TCR_SSR.g{2} k)); 1,2: by smt().
-  - by call Eqv_fixone_if_dfc.
-  inline *.
-  wp; sp.
-  rnd; rnd.
-  by skip. 
-wp.
-call (:   TCR_SS.k0{1} = TCR_SSR.k0{2} 
-       /\ TCR_SS.O_TCR_SS.g{1} 
-          =
-          (fun (k : key) =>
-            if k = TCR_SSR.k0{2}
-            then TCR_SSR.gk{2}
-            else TCR_SSR.g{2} k)).
-+ proc; inline *.
-  by wp; skip.
-wp.
-call (: TCR_SS.O_TCR_SS.g{1} 
-        =
-        (fun (k : key) =>
-          if k = TCR_SSR.k0{2} 
-          then TCR_SSR.gk{2}
-          else TCR_SSR.g{2} k)).
-+ by proc; inline *; wp; skip.
-by skip.
-qed.
-
-
-local lemma EqPr_TCR_TCRSSR &m:
-  Pr[TCR(A, O_Default).main() @ &m : res]
-  =
-  Pr[TCR_SSR.main() @ &m : res].
-proof. 
-by rewrite EqPr_TCR_TCRSS EqPr_TCRSS_TCRSSR. 
-qed.
-
-
-local module TCR_SSR_Nin = {
-  var k0 : key
-  var ks : key list
-  var gk : input -> output
-  var g : key -> input -> output
-  
-  module O_TCR_SSR_Pick : Oracle_t = {  
-    proc get(k : key, x : input) = {
-      ks <- rcons ks k;
-      
-      return g k x;
-    }
-  }
-
- module O_TCR_SSR_Find : Oracle_t = {  
-    proc get(k : key, x : input) = {
-      var y : output;
-      
-      if (k = k0) {
-        y <- gk x;
-      } else {
-        y <- g k x;
-      } 
-      
-      return y;
-    }
-  }
-  
-  proc main() : bool = {
-    var x, x' : input;
-    var y, y' : output;
-    
-    k0 <$ dkey;
-    
-    ks <- [];
-    
-    gk <$ dfcs;  
-    g <$ dfc;
-    
-    x <@ A(O_TCR_SSR_Pick).pick();
-    y <@ O_TCR_SSR_Find.get(k0, x);
-    
-    x' <@ A(O_TCR_SSR_Find).find(k0);
-    y' <@ O_TCR_SSR_Find.get(k0, x');
-    
-    return x' <> x /\ y' = y;
-  }
-}.
-
-
-local lemma LePr_TCRSSR_In &m :
-  Pr[TCR_SSR.main() @ &m : res /\ (TCR_SSR.k0 \in TCR_SSR.ks)]
-  <=
-  Pr[TCR_SSR.main() @ &m : (TCR_SSR.k0 \in TCR_SSR.ks)].
-proof. by byequiv (: _ ==> ={TCR_SSR.k0, TCR_SSR.ks}) => //; sim. qed.
-
-local lemma EqPr_TCRSSR_TCRSSRNin &m:
-  Pr[TCR_SSR.main() @ &m : res /\ ! (TCR_SSR.k0 \in TCR_SSR.ks)]
-  =
-  Pr[TCR_SSR_Nin.main() @ &m : res /\ ! (TCR_SSR_Nin.k0 \in TCR_SSR_Nin.ks)].
-proof. 
-byequiv (: (res /\ ! (TCR_SSR.k0 \in TCR_SSR.ks)){1}
-           <=>
-           (res /\ ! (TCR_SSR_Nin.k0 \in TCR_SSR_Nin.ks)){2}) => //.
-proc; inline *.
-wp => /=.
-seq 4 4 : (   ={glob A} 
-           /\ ={k0, ks, gk, g}(TCR_SSR, TCR_SSR_Nin)
-           /\ TCR_SSR.ks{1} = []); 1: by auto.
-seq 1 1 : (   ={k0, gk, g}(TCR_SSR, TCR_SSR_Nin)
-           /\ (TCR_SSR.k0{1} \in TCR_SSR.ks{1} <=> TCR_SSR_Nin.k0{2} \in TCR_SSR_Nin.ks{2})
-           /\ (! (TCR_SSR_Nin.k0{2} \in TCR_SSR_Nin.ks{2}) 
-               => 
-               ={glob A, x} /\ ={ks}(TCR_SSR, TCR_SSR_Nin))).
-+ call (: TCR_SSR_Nin.k0 \in TCR_SSR_Nin.ks, 
-        ={k0, ks, gk, g}(TCR_SSR, TCR_SSR_Nin), 
-        ={k0, gk, g}(TCR_SSR, TCR_SSR_Nin)
-        /\
-        TCR_SSR.k0{1} \in TCR_SSR.ks{1}
-        <=>
-        TCR_SSR_Nin.k0{2} \in TCR_SSR_Nin.ks{2}).
-+ by move=> O Oll; move: (A_pick_ll O Oll).
-+ proc.
-  case (k{2} = TCR_SSR_Nin.k0{2}).
-  - wp; skip => />; smt(mem_rcons).
-  by wp; skip => />.
-+ move=> &2 k0in.
-  proc.
-  wp; skip => />; smt(mem_rcons).
-+ move=> &1.
-  proc.
-  by wp; skip => />; smt(mem_rcons).
-+ by skip => /> /#.
-case (TCR_SSR_Nin.k0{2} \in TCR_SSR_Nin.ks{2}).
-+ conseq (: _ ==> true); 1: by smt().
-  call{1} (: true ==> true); 2: call{2} (: true ==> true).
-  - apply (A_find_ll TCR_SSR.O_TCR_SSR_Find).
-    by proc; wp.     
-  - apply (A_find_ll TCR_SSR_Nin.O_TCR_SSR_Find).
-    by proc; wp.
-  by wp; skip.
-call (: ={k0, gk, g}(TCR_SSR, TCR_SSR_Nin)).
-+ proc.
-  by wp; skip.
-by wp; skip => /> /#.
-qed.
-
-local module TCR_Rep = {
-  var k0 : key
-  var x0 : input
-  var y0 : output
-  var ks : key list
-  var gk : input -> output
-  var g : key -> input -> output
-  
-  module O_TCR_Rep_Pick : Oracle_t = {
-    proc get(k : key, x : input) : output = {
-      var b : bool;
-      var y : output;
-      
-      ks <- rcons ks k;
-      
-      return g k x;
-    }
-  }
-
-  module O_TCR_Rep_Find : Oracle_t = {
-    proc get(k : key, x : input) : output = {
-      var b : bool;
-      var y : output;
-      
-      if (k = k0) {
-        b <@ BFOF.query(x);
-        y <- if !b /\ x <> x0 then gk x else y0;
-      } else { 
-        y <- g k x;
-      }
-      
-      return y;
-    }
-  }
-
-  proc main() : bool = {
-    var x' : input;
-    var y' : output;
-    
-    BFOF.init();
-    
-    ks <- [];
-    
-    k0 <$ dkey;
-    y0 <$ doutput;
-    
-    gk <$ MUFF_In.dfun (fun _ => doutput \ (pred1 y0));    
-    g <$ dfc;
-    
-    x0 <@ A(O_TCR_Rep_Pick).pick();
-        
-    x' <@ A(O_TCR_Rep_Find).find(k0);
-    
-    y' <@ O_TCR_Rep_Find.get(k0, x');
-    
-    return x' <> x0 /\ y' = y0;
-  }
-}.
-
-
-local lemma TCRSPRNin_Implies_TCRRep &m :
-  Pr[TCR_SSR_Nin.main() @ &m : res /\ ! (TCR_SSR_Nin.k0 \in TCR_SSR_Nin.ks)]
-  <=
-  Pr[TCR_Rep.main() @ &m : res].
-proof.
-byequiv=> //.
-proc; inline *.
-swap{2} [2..3] -1.
-swap{1} [4..5] -1; swap{2} [6..7] -3; swap{2} 6 -1.
-seq 4 4 : (   ={glob A} 
-           /\ ={k0, ks, g}(TCR_SSR_Nin, TCR_Rep)
-           /\ x{1} = TCR_Rep.x0{2}).
-+ call (: ={ks, g}(TCR_SSR_Nin, TCR_Rep)); 1: by proc; wp.
-  by rnd; wp; rnd; wp; skip.
-wp => /=.
-seq 1 3 : (   #pre 
-           /\ (forall (x : input),
-                 TCR_SSR_Nin.gk{1} x
-                 =
-                 if !BFOF.f{2} x /\ x <> TCR_Rep.x0{2} 
-                 then TCR_Rep.gk{2} x
-                 else TCR_Rep.y0{2})).
-conseq (: _ 
-          ==> 
-          (forall (x : input),
-             TCR_SSR_Nin.gk{1} x
-             =
-             if !BFOF.f{2} x /\ x <> TCR_Rep.x0{2} 
-             then TCR_Rep.gk{2} x
-             else TCR_Rep.y0{2})) => //.
-+ transitivity{1} {TCR_SSR_Nin.gk <@ LR.LambdaRepro.left();}
-                  (true ==> ={TCR_SSR_Nin.gk})
-                  (x{1} = TCR_Rep.x0{2} 
-                   ==>
-                   (forall (x : input),
-                     TCR_SSR_Nin.gk{1} x 
-                     =
-                     if !BFOF.f{2} x /\ x <> TCR_Rep.x0{2} 
-                     then TCR_Rep.gk{2} x
-                     else TCR_Rep.y0{2})); 1,2: by smt().
-  - inline *.
-    by wp; rnd.
-  transitivity{1} {TCR_SSR_Nin.gk <@ LR.LambdaRepro.right(x);}
-                  (true ==> ={TCR_SSR_Nin.gk})
-                  (x{1} = TCR_Rep.x0{2} 
-                   ==> 
-                   (forall (x : input),
-                     TCR_SSR_Nin.gk{1} x 
-                     =
-                     if !BFOF.f{2} x /\ x <> TCR_Rep.x0{2} 
-                     then TCR_Rep.gk{2} x
-                     else TCR_Rep.y0{2})); 1,2: by smt().
-  - by call LR.main_theorem.
-  inline *.
-  by wp; rnd; rnd; rnd; wp; skip.
-call (:   ={k0, ks, g}(TCR_SSR_Nin, TCR_Rep)
-       /\ (forall (x : input),
-             TCR_SSR_Nin.gk{1} x 
-             =
-             if !BFOF.f{2} x /\ x <> TCR_Rep.x0{2} 
-             then TCR_Rep.gk{2} x
-             else TCR_Rep.y0{2})).
-+ proc; inline *.
-  by wp; skip => /> /#.
-by wp; skip => /> /#. 
-qed.
-
-
-local lemma TCRRepNin_Implies_BFFind &m :
-  Pr[TCR_Rep.main() @ &m : res]
-  <=
-  Pr[BF_Find(R_BFFind_TCR(A), BFOF).main() @ &m: res].
-proof.
-byequiv=> //.
-proc; inline *.
-wp => /=.
-call (:   ={BFOF.f}
-       /\ ={k0, x0, y0, g}(TCR_Rep, R_BFFind_TCR)
-       /\ TCR_Rep.gk{1} = R_BFFind_TCR.f{2}). 
-+ proc; inline *.
-  by wp; skip.
-call (: ={g}(TCR_Rep, R_BFFind_TCR)).
-+ proc.
-  by wp; skip.
-do 4! rnd; wp; rnd; skip => /> f ? ? ? y ? gk gkin ? ? ? r ?.
-apply contraLR => -> /=.
-by move/dfun_supp /(_ r) /supp_dexcepted: gkin.
-qed.
-
-local lemma TCR_Implies_BFDistinguish_A &m:
-  Pr[KHFO_TCR.TCR(A, KHFO.O_Default).main() @ &m : res]
-  <=
-  `| Pr[BF_Distinguish(R_BFDistinguish_BFFind(R_BFFind_TCR(A)), BFOD).main(false) @ &m : res] - 
-     Pr[BF_Distinguish(R_BFDistinguish_BFFind(R_BFFind_TCR(A)), BFOD).main(true) @ &m : res] |
-  +
-  Pr[TCR_SSR.main() @ &m : (TCR_SSR.k0 \in TCR_SSR.ks)].
-proof.
-apply (StdOrder.RealOrder.ler_trans 
-          (Pr[BF_Find(R_BFFind_TCR(A), BFOF).main() @ &m : res] +
-           Pr[TCR_SSR.main() @ &m : (TCR_SSR.k0 \in TCR_SSR.ks)])); last first.
-+ by rewrite (Find_Implies_Distinguish &m (R_BFFind_TCR(A))).
-rewrite EqPr_TCR_TCRSSR Pr[mu_split (! TCR_SSR.k0 \in TCR_SSR.ks)] /= StdOrder.RealOrder.ler_add.
-+ rewrite EqPr_TCRSSR_TCRSSRNin (StdOrder.RealOrder.ler_trans Pr[TCR_Rep.main() @ &m : res]).
-  - by apply TCRSPRNin_Implies_TCRRep.
-  by apply TCRRepNin_Implies_BFFind.
-by apply LePr_TCRSSR_In.
-qed.
-
-
-(* Query counting *)
-declare op q : { int | 0 <= q } as ge0_q.
-
-declare axiom A_pick_qs (O <: Oracle_t{-A}) (n : int) :
-  hoare[A(Counting_O(O)).pick : Counting_O.ctr = n ==> Counting_O.ctr <= n + q].
-
-
-local module TCR_SSR_C = {
-  import var TCR_SSR   
- 
-  module O_TCR_SSR_C_Pick : Oracle_t = {
-    proc get(k : key, x : input) = {
-      var y : output;
-      
-      ks <- if size ks < q then rcons ks k else ks;
-      
-      if (k = k0) { 
-        y <- gk x;
-      } else { 
-        y <- g k x;
-      }
-      
-      return y;
-    }
-  }
-  
-  module O_TCR_SSR_C_Find : Oracle_t = TCR_SSR.O_TCR_SSR_Find
-   
-  proc main() : bool = {
-    var x, x' : input;
-    var y, y' : output;
-    
-    Counting_O.ctr <- 0;
-    ks <- [];
-    
-    k0 <$ dkey;
-    
-    gk <$ dfcs;  
-    g <$ dfc;
-    
-    x <@ A(Counting_O(O_TCR_SSR_C_Pick)).pick();
-    y <@ O_TCR_SSR_C_Find.get(k0, x);
-    
-    x' <@ A(O_TCR_SSR_C_Find).find(k0);
-    y' <@ O_TCR_SSR_C_Find.get(k0, x');
-    
-    return x' <> x /\ y' = y;
-  }
-}.
-
-(* 
-  The following only works due to the fact that O_TCR_SSR_C_Pick still returns 
-  the same values after q queries have been issued (as it returns before q queries are issued). 
-  I want this to be cleaner:
-  I want O_TCR_SSR_C_Pick to simply return an error/witness whenever the size of the
-  list of keys (ks) has reached q (i.e., q queries have been issued).
-  The following lemma should then still hold simply because, by assumption, it should 
-  be impossible for the size of ks to already be q in a query, as the adversary 
-  is assumed to not query more than q times (Counting_O.ctr <= q, and size ks is invariably
-  the same as Counting_O.ctr up until reaching q).
-  However, I cannot get this to work.
-*)
-local lemma EqPr_TCRSSR_TCRSSRC &m:
-  Pr[TCR_SSR.main() @ &m : (TCR_SSR.k0 \in TCR_SSR.ks)]
-  =
-  Pr[TCR_SSR_C.main() @ &m : (TCR_SSR.k0 \in TCR_SSR.ks)].
-proof.
-(*
-rewrite Pr[mu_split (size TCR_SSR.ks <= q)] eq_sym Pr[mu_split (Counting_O.ctr <= q)] eq_sym.
-congr. admit.
-rewrite 2!lezNgt /=.
-byequiv=> //=.
-proc; inline *.
-seq 4 5 : (   ={glob A, TCR_SSR.k0, TCR_SSR.ks, TCR_SSR.gk, TCR_SSR.g}
-           /\ TCR_SSR.ks{1} = []
-           /\ Counting_O.ctr{2} = 0); 1: by auto.
-wp => /=.
-call (: true).
-
-           seq 1 1 : (   ={glob A, TCR_SSR.k0, TCR_SSR.gk, TCR_SSR.g}
-           /\ TCR_SSR.ks{1} = []
-           /\ Counting_O.ctr{2} = 0
-           rewrite eq_sym Pr[mu_split (Counting_O.ctr <= q)] eq_sym.
-*)
-rewrite eq_sym Pr[mu_split (Counting_O.ctr <= q)] eq_sym.
-rewrite -(StdOrder.RealOrder.Domain.addr0 Pr[TCR_SSR.main() @ &m : TCR_SSR.k0 \in TCR_SSR.ks]).
-congr; last first.
-+ byphoare => //.
-  hoare.
-  conseq (: _ ==> Counting_O.ctr <= q); 1: by smt().
-  proc; inline *.
-  wp.
-  call (: true); 1: by proc; wp; skip.
-  wp.
-  call (A_pick_qs TCR_SSR_C.O_TCR_SSR_C_Pick 0).
-  by do 3! rnd; wp; skip. 
-byequiv => //.
-proc; inline *.
-wp => /=.
-call{1} (: true ==> true); 2: call{2} (: true ==> true).
-+ apply (A_find_ll TCR_SSR.O_TCR_SSR_Find).
-  by proc; wp.     
-+ apply (A_find_ll TCR_SSR_C.O_TCR_SSR_C_Find).
-  by proc; wp.
-wp => /=.
-call (:   ={glob A, TCR_SSR.gk, TCR_SSR.k0, TCR_SSR.g, TCR_SSR.ks}
-       /\ Counting_O.ctr{2} = 0
-       /\ size TCR_SSR.ks{2} = 0
-       ==>
-          ={TCR_SSR.gk, TCR_SSR.k0, TCR_SSR.g} 
-       /\ Counting_O.ctr{2} <= q
-       /\ (Counting_O.ctr{2} <= q => 
-             ={TCR_SSR.ks} /\
-             Counting_O.ctr{2} = size TCR_SSR.ks{2})).
-+ conseq (:    ={glob A, TCR_SSR.gk, TCR_SSR.k0, TCR_SSR.g, TCR_SSR.ks}
-            /\ Counting_O.ctr{2} = 0 /\ size TCR_SSR.ks{2} = 0
-            ==>
-               ={TCR_SSR.gk, TCR_SSR.k0, TCR_SSR.g}
-            /\ (Counting_O.ctr{2} <= q => 
-                   size TCR_SSR.ks{2} = Counting_O.ctr{2}
-                /\ ={TCR_SSR.ks})) 
-         (: true ==> true)
-         (A_pick_qs TCR_SSR_C.O_TCR_SSR_C_Pick 0) => //. smt().
-  proc (={TCR_SSR.gk, TCR_SSR.k0, TCR_SSR.g}
-            /\ (Counting_O.ctr{2} <= q => 
-                   size TCR_SSR.ks{2} = Counting_O.ctr{2}
-                /\ ={TCR_SSR.ks})).
-  smt().
-  smt().
-  proc.
-  inline *.
-  wp. skip => />. progress. smt(size_rcons).
-         smt(size_rcons). smt(size_rcons). smt(size_rcons). 
-by rnd; rnd; wp; rnd; wp; skip => />. 
-qed.
-
-(*
-local lemma EqPr_TCRSSR_TCRSSRC &m:
-  Pr[TCR_SSR.main() @ &m : (TCR_SSR.k0 \in TCR_SSR.ks)]
-  =
-  Pr[TCR_SSR_C.main() @ &m : (TCR_SSR.k0 \in TCR_SSR.ks)].
-proof.
-byequiv => //.
-proc; inline *.
-seq 5 6 : (   ={glob A, TCR_SSR.gk, TCR_SSR.k0, TCR_SSR.g, TCR_SSR.ks}); last first.
-+ by conseq (: _ ==> true) => //; sim.
-call (: ={TCR_SSR.gk, TCR_SSR.k0, TCR_SSR.g, TCR_SSR.ks}).
-+ proc; inline *.
-  by wp; skip.
-(*
-call (:   ={glob A, TCR_SSR.gk, TCR_SSR.k0, TCR_SSR.g, TCR_SSR.ks}
-       /\ Counting_O.ctr{2} = 0
-       ==>
-          ={glob A, TCR_SSR.gk, TCR_SSR.k0, TCR_SSR.g, TCR_SSR.ks} 
-       /\ Counting_O.ctr{2} <= q).
-+ conseq (: ={glob A, TCR_SSR.gk, TCR_SSR.k0, TCR_SSR.g, TCR_SSR.ks}
-            ==>
-            ={glob A, TCR_SSR.gk, TCR_SSR.k0, TCR_SSR.g, TCR_SSR.ks}) 
-         (: true ==> true)
-         (A_pick_qs TCR_SSR.O_TCR_SSR_Pick 0) => //.
-  proc (={TCR_SSR.gk, TCR_SSR.k0, TCR_SSR.g, TCR_SSR.ks}) => //.
-  proc; inline *.
-  by wp; skip.
-*)
-by rnd; rnd; wp; rnd; wp; skip.
-qed.
-*)
-
-
-(* Check LeakyEager/SuperEager; fel doesn't work *)
-local lemma Bound_TCRSSRC &m:
- Pr[TCR_SSR_C.main() @ &m : (TCR_SSR.k0 \in TCR_SSR.ks)]
- <=
- q%r * mu1 witness dkey.
-proof.
-print TCR_SSR_C.
-fel 3
-    (size TCR_SSR.ks) 
-    (fun (i : int) => mu1 witness dkey) 
-    q 
-    (TCR_SSR.k0 \in TCR_SSR.ks)
-    [TCR_SSR_C.O_TCR_SSR_C_Pick.get : (size TCR_SSR.ks < q)]
-    (size TCR_SSR.ks <= q).
-by rewrite (: q%r = (q - 0)%r) 1:// StdBigop.Bigreal.sumri_const 1:ge0_q.
-smt().
-rnd; wp; skip => />. by rewrite ge0_q.
-proc.
-(* Move sampling to oracle procedure? *) 
-admit.
-move=> c.
-proc. 
-wp; skip => />.  smt(size_rcons).
-move=> b c.
-proc. by wp; skip => />.
-qed.
-
-local lemma TCR_Implies_BFDistinguish &m:
-  Pr[KHFO_TCR.TCR(A, KHFO.O_Default).main() @ &m : res]
-  <=
-  `| Pr[BF_Distinguish(R_BFDistinguish_BFFind(R_BFFind_TCR(A)), BFOD).main(false) @ &m : res] - 
-     Pr[BF_Distinguish(R_BFDistinguish_BFFind(R_BFFind_TCR(A)), BFOD).main(true) @ &m : res] |
-  +
-  q%r * mu1 witness dkey.
-proof.
-move: (TCR_Implies_BFDistinguish_A &m); rewrite EqPr_TCRSSR_TCRSSRC.
-by move: (Bound_TCRSSRC &m) => /#.
-qed.
-end section.
-*)
-
-(*
-section.
-
-declare module A <: Adv_TCR {-KHFO.O_Default, -BFOF, -BFOD, -R_BFFind_TCR, -Counting_O}.
-
-declare axiom A_pick_ll (O <: Oracle_t{-A}):
-  islossless O.get => islossless A(O).pick.
-
-declare axiom A_find_ll (O <: Oracle_t{-A}):
-  islossless O.get => islossless A(O).find.
-
-
-local clone import DFun as DF with
-  type in_t <- key,
-  type out_t <- input -> output,
-    op dout <- dfcs,
-    
-  theory FT_In <- FinKey
-  
-  proof *.
-  realize dout_ll by exact: dfcs_ll.
-
-local clone import Reprogramming as Repro with
-  type in_t <- key,
-  type out_t <- input -> output,
-    op dout <- dfcs,
-    
-  theory FT_In <- FinKey
-  
-  proof *.
-  realize dout_ll by exact: dfcs_ll.
-
-import LE.
-
-require import SmtMap.
-
-local module TCR_Fmap_Rep = {
-  module O_TCR_Fmap_Rep : Oracle_t = {
-    var m : (key, input -> output) fmap
-    var g : key -> input -> output
-    
-    proc init() : unit = {
-      var y : input -> output;
-      var w : key list;
-      var k : key;
-      
-      m <- empty;
-      w <- FinKey.enum;
-      while (w <> []){
-        k <- head witness w;
-        y <$ dfcs;
-        m.[k] <- y;
-        w <- behead w;
-      }
-      
-      g <- fun (k : key) => oget m.[k];
-    }
-    
-    proc get(k : key, x : input) : output = {
-      return g k x;
-    }
-  }
-  
-  proc main() = {
-    var k : key;
-    var x, x' : input;
-    var y, y' : output;
-    
-    BFOF.init();
-    O_TCR_Fmap.init();
-    
-    x <@ A(O_TCR_Fmap).pick();
-    
-    k <$ dkey;
-    
-    O_TCR_Fmap_Rep <-
-    
-    y <@ O_TCR_Fmap.get(k, x);
-        
-    x' <@ A(O_TCR_Fmap).find(k);
-    y' <@ O_TCR_Fmap.get(k, x');
-    
-    return x' <> x /\ y' = y;
-  }
-}.
-
-local equiv Eqv_TCR_TCR_Fmap :
-  KHFO_TCR.TCR(A, O_Default).main ~ TCR_Fmap.main :
-    ={glob A} ==> ={res}.
-proof.
-proc.
-inline *.
-seq 1 4: (={glob A} /\ O_Default.f{1} = TCR_Fmap.O_TCR_Fmap.g{2}).
-+ transitivity{1} {O_Default.f <$ dfc;}
-                  (={glob A} ==> ={glob A} /\ ={O_Default.f})
-                  (={glob A} ==> ={glob A} /\ O_Default.f{1} = TCR_Fmap.O_TCR_Fmap.g{2}); 1,2:  by smt().
-  - by rnd; skip => /=; rewrite eq_df_dfc.
-  transitivity{1} {O_Default.f <@ Direct.sample();}
-                  (={glob A} ==> ={glob A} /\ ={O_Default.f})
-                  (={glob A} ==> ={glob A} /\ O_Default.f{1} = TCR_Fmap.O_TCR_Fmap.g{2}); 1,2:  by smt().
-  - inline *. 
-    by wp; rnd; skip.
-  wp.
-  transitivity{2} {TCR_Fmap.O_TCR_Fmap.m <@ Loop_Fmap_Head.sample();}
-                  (={glob A} ==> ={glob A} /\ O_Default.f{1} = fun (k' : key) => oget TCR_Fmap.O_TCR_Fmap.m{2}.[k'])
-                  (={glob A} ==> ={glob A} /\ ={TCR_Fmap.O_TCR_Fmap.m}); 1,2: by smt().
-  - symmetry.
-    conseq (: ={glob A} 
-              ==> 
-                 ={glob A} 
-              /\ (fun (k' : key) => oget TCR_Fmap.O_TCR_Fmap.m{1}.[k']) = O_Default.f{2}) => //.
-    call Eqv_Loop_Fmap_Head_Direct_Map.
-    by skip.
-  inline *.
-  by wp; swap{1} 1 1; sim.
-wp.
-call (: O_Default.f{1} = TCR_Fmap.O_TCR_Fmap.g{2}).
-+ by proc.
-wp; rnd.
-call (: O_Default.f{1} = TCR_Fmap.O_TCR_Fmap.g{2}).
-+ by proc.
-by skip.
-qed.
-
-
-local module TCR_ERO = {
-  module O_TCR_ERO : Oracle_r = {
-    var m : (key, input -> output) fmap
-    var g : key -> input -> output
-    
-    proc init() : unit = {
-      var y : input -> output;
-      var w : key list;
-      var k : key;
-      
-      m <- empty;
-      w <- FinKey.enum;
-      while (w <> []){
-        k <- head witness w;
-        y <$ dfcs;
-        m.[k] <- y;
-        w <- behead w;
-      }
-      
-      g <- fun (k : key) => oget m.[k];
-    }
-    
-    proc get(k : key, x : input) : output = {
-      return g k x;
-    }
-  }
-  
-  proc main() = {
-    var k : key;
-    var x, x' : input;
-    var y, y' : output;
-    
-    O_TCR_Fmap.init();
-    
-    x <@ A(O_TCR_Fmap).pick();
-    
-    k <$ dkey;
-    
-    y <@ O_TCR_Fmap.get(k, x);
-        
-    x' <@ A(O_TCR_Fmap).find(k);
-    y' <@ O_TCR_Fmap.get(k, x');
-    
-    return x' <> x /\ y' = y;
-  }
-}.
-
-local module TCR_ERO_Rep = {
-  var k0 : key
-  
-  module O_TCR_ERO : Oracle_t = {
-    var g : key -> input -> output
-    
-    proc init() : unit = {
-      g <$ dfc;
-    }
-    
-    proc get(k : key, x : input) : output = {
-      return g k x;
-    }
-  }
-  
-  proc main() = {
-    var x, x' : input;
-    var y, y' : output;
-    
-    O_TCR_ERO.init();
-    
-    k0 <$ dkey;
-    
-    x <@ A(O_TCR_ERO).pick();
-    y <@ O_TCR_ERO.get(k0, x);
-        
-    x' <@ A(O_TCR_ERO).find(k0);
-    y' <@ O_TCR_ERO.get(k0, x');
-    
-    return x' <> x /\ y' = y;
-  }
-}.
-
-
-
-
-
-end section.
-*)
