Reprogramming.ec
@@ -29,16 +29,16 @@ clone import ROM_.LazyEager as LE with
   
   proof *.
   
-module type Oracle_r = {
-    include Oracle
-    proc set(x : in_t, y : out_t) : unit
+module type Oracleip_t = {
+  include Oracle
+  proc set(x : in_t, y : out_t) : unit
 }.
 
-module type POracle_r = {
-    include Oracle_r [-init]
+module type Oraclep_t = {
+  include Oracleip_t [-init]
 }.
 
-module Wrapped_Oracle (O: POracle) : Oracle_r = {
+module O_Programmable(O : POracle) : Oraclep_t = {
    var prog_list : (in_t * out_t) list  
    var ch : int
 
@@ -48,78 +48,86 @@ module Wrapped_Oracle (O: POracle) : Oracle_r = {
    }
 
   proc o(x : in_t): out_t = {
-     var r,c : out_t;
-     var tmp : out_t option;
-    
-     r <@ O.o(x);
+    var r,c : out_t;
+    var tmp : out_t option;
 
-     ch <- ch + 1; 
-     tmp <- assoc prog_list x;
-     c <- if tmp = None then r else oget tmp;
-     return c; 
+    r <@ O.o(x);
+
+    ch <- ch + 1; 
+    tmp <- assoc prog_list x;
+    c <- if tmp = None then r else oget tmp;
+
+    return c; 
   }
 
    proc set (x : in_t, y: out_t) : unit = {
      prog_list <- (x,y) :: prog_list;
    }
-
 }.
 
-module type RepO_ti = {
-    proc init(b : bool) : unit
-    proc repro(p : pT) : in_t
+module type Oracleir_t = {
+  proc init(b : bool) : unit
+  proc repro(p : pT) : in_t
 }.
 
-module type RepO_t = {
-    include RepO_ti [-init]
+module type Oracler_t = {
+  include Oracleir_t [-init]
 }.
 
-module RepO(RO: POracle_r) : RepO_ti = {
-    var ctr : int
-    var b : bool
-    var se : bool
 
-    proc init(in_b : bool) : unit = {
-        ctr <- 0;
-        b <- in_b;
-        se <- true;
+module O_Reprogrammer(O : Oraclep_t) : Oracler_t = {
+  var ctr : int
+  var b : bool
+  var se : bool
+
+  proc init(in_b : bool) : unit = {
+    ctr <- 0;
+    b <- in_b;
+    se <- true;
+  }
+
+  proc repro(p: pT) : in_t = {
+    var x : in_t;
+    var y : out_t;
+
+    se <- if p_max p <= p_max_bound then se else false;
+    ctr <- ctr + 1;
+
+    x <$ p;
+
+    if (b) {
+      y <$ dout;
+      O.set(x,y);
     }
 
-    proc repro(p: pT) : in_t = {
-        var x,y;
-        se <- if p_max p <= p_max_bound then se else false;
-        ctr <- ctr + 1;
-        x <$ p;
-        if (b) {
-            y <$ dout;
-            RO.set(x,y);
-        } 
-        return x;
-    }
+    return x;
+  }
 }.
 
-module type DistA(RO: POracle, O: RepO_t) = {
-    proc distinguish() : bool {RO.o, O.repro}
+module type Adv_INDRepro(O : Oraclep_t, OR : Oracler_t) = {
+  proc distinguish() : bool {O.o, OR.repro}
 }.
 
-
-module ReproGame(RO : Oracle, A : DistA) = {
-  module Wrap = Wrapped_Oracle(RO)
-  module O = RepO(Wrap)
+module IND_Repro(O : Oracle, A : Adv_INDRepro) = {
+  module OP = O_Programmable(O)
+  module OR = O_Reprogrammer(OP)
  
-  proc main (b: bool) : bool = {
-    var b';
-    RO.init();
-    Wrap.init();
-    O.init(b);
-    b' <@ A(Wrap, O).distinguish();
+  proc main (b : bool) : bool = {
+    var b' : bool;
+    
+    O.init();
+    OP.init();
+    OR.init(b);
+    
+    b' <@ A(OP, OR).distinguish();
+    
     return b';
   } 
 }.
 
 section.
 
-declare module A <: DistA {-ReproGame, -ERO, -Lazy.LRO}.
+declare module A <: Adv_INDRepro {-IND_Repro, -ERO, -Lazy.LRO}.
 
 declare const rep_ctr : {int | 0 <= rep_ctr } as ge0_repctr.
 declare const query_ctr : {int | 0 <= query_ctr } as ge0_queryctr.
@@ -131,16 +139,16 @@ local module Bad = {
   var i  : int
 }.
 
-local module Wrapped_Oracle1 (O: POracle) : Oracle_r = {
-  include var Wrapped_Oracle(O) [-o]
+local module O_Programmable1 (O : POracle) : Oracleip_t = {
+  include var O_Programmable(O) [-o]
   import var Bad
  
   proc o(x : in_t): out_t = {
-    var r,c : out_t;
+    var r, c : out_t;
     var tmp : out_t option;
 
     c <- witness;
-    if (co <  query_ctr) { 
+    if (co < query_ctr) { 
       r <@ O.o(x);
       tmp <- assoc prog_list x;
       c <- if tmp = None then r else oget tmp;
@@ -152,22 +160,24 @@ local module Wrapped_Oracle1 (O: POracle) : Oracle_r = {
       c <- if tmp = None then r else oget tmp;      
       co <- co + 1;
     }
+    
     ch <- ch + 1; 
+    
     return c; 
   }
 
 }.
 
-local module Wrapped_Oracle2 (O: POracle) : Oracle_r = {
-  include var Wrapped_Oracle(O) [-o]
+local module O_Programmable2 (O: POracle) : Oracleip_t = {
+  include var O_Programmable(O) [-o]
   import var Bad
  
   proc o(x : in_t): out_t = {
-    var r,c : out_t;
+    var r, c : out_t;
     var tmp : out_t option;
 
     c <- witness;
-    if (co <  query_ctr) { 
+    if (co < query_ctr) { 
       r <@ O.o(x);
       tmp <- assoc prog_list x;
       c <- if tmp = None then r else oget tmp;
@@ -175,18 +185,20 @@ local module Wrapped_Oracle2 (O: POracle) : Oracle_r = {
     } else {
       bad <- true;
     }
+    
     ch <- ch + 1; 
+    
     return c; 
   }
 
 }.
 
-local module Wrapped_Oracle2' (O: POracle) : Oracle_r = {
-  include var Wrapped_Oracle(O) [-o]
+local module O_Programmable2S (O: POracle) : Oracleip_t = {
+  include var O_Programmable(O) [-o]
   import var Bad
 
   proc o(x : in_t): out_t = {
-    var r,c : out_t;
+    var r, c : out_t;
     var tmp : out_t option;
 
     c <- witness;
@@ -196,25 +208,30 @@ local module Wrapped_Oracle2' (O: POracle) : Oracle_r = {
       c <- if tmp = None then r else oget tmp;
       co <- co + 1;
     } 
+
     ch <- ch + 1; 
+    
     return c; 
   }
 
 }.
 
-local module RepO1(RO: POracle_r) : RepO_ti = {
-  include var RepO(RO) [-repro]
+local module O_Reprogrammer1(O: Oraclep_t) : Oracleir_t = {
+  include var O_Reprogrammer(O) [-repro]
   import var Bad
 
-  proc repro(p: pT) : in_t = {
-    var x,y;
+  proc repro(p : pT) : in_t = {
+    var x : in_t;
+    var y : out_t;
+    
     se <- if p_max p <= p_max_bound then se else false;
+    
     x <- witness;
     if (se /\ cr < rep_ctr) { 
       x <$ p;
       if (b) {
         y <$ dout;
-        RO.set(x,y);
+        O.set(x, y);
       }
       cr <- cr + 1;
     } else { 
@@ -222,271 +239,361 @@ local module RepO1(RO: POracle_r) : RepO_ti = {
       x <$ p;
       if (b) {
         y <$ dout;
-        RO.set(x,y);
+        O.set(x, y);
       }
       cr <- cr + 1;
     }
+    
     ctr <- ctr + 1;
+    
     return x;
   }
 }.
 
-local module RepO2(RO: POracle_r) : RepO_ti = {
-  include var RepO(RO) [-repro]
+local module O_Reprogrammer2(O: Oraclep_t) : Oracleir_t = {
+  include var O_Reprogrammer(O) [-repro]
   import var Bad
 
-  proc repro(p: pT) : in_t = {
+  proc repro(p : pT) : in_t = {
     var x,y;
+    
     se <- if p_max p <= p_max_bound then se else false;
+    
     x <- witness;
     if (se /\ cr < rep_ctr) { 
       x <$ p;
       if (b) {
         y <$ dout;
-        RO.set(x,y);
+        O.set(x,y);
       } 
       cr <- cr + 1;
     } else { 
       bad <- true;
     }
+    
     ctr <- ctr + 1;
+    
     return x;
   }
 }.
 
-local module ReproGame1 (RO: Oracle, A: DistA) = {
+local module IND_Repro1 (O: Oracle, A: Adv_INDRepro) = {
   import var Bad
-  module Wrap = Wrapped_Oracle1(RO)
-  module O = RepO1(Wrap)
+  
+  module OP = O_Programmable1(O)
+  module OR = O_Reprogrammer1(OP)
  
-  proc main (b: bool) : bool = {
-    var b';
+  proc main (b : bool) : bool = {
+    var b' : bool;
+    
     bad <- false; co <- 0; cr <- 0;
-    RO.init();
-    Wrap.init();
-    O.init(b);
-    b' <@ A(Wrap, O).distinguish();
+    
+    O.init();
+    OP.init();
+    OR.init(b);
+    
+    b' <@ A(OP, OR).distinguish();
+    
     return b';
   } 
 }.
 
-local module ReproGame2 (RO: Oracle, A: DistA) = {
+local module IND_Repro2 (O: Oracle, A: Adv_INDRepro) = {
   import var Bad
-  module Wrap = Wrapped_Oracle2(RO)
-  module O = RepO2(Wrap)
+  
+  module OP = O_Programmable2(O)
+  module OR = O_Reprogrammer2(OP)
  
-  proc main (b: bool) : bool = {
-    var b';
+  proc main (b : bool) : bool = {
+    var b' : bool;
+    
     bad <- false; co <- 0; cr <- 0;
-    RO.init();
-    Wrap.init();
-    O.init(b);
-    b' <@ A(Wrap, O).distinguish();
+    
+    O.init();
+    OP.init();
+    OR.init(b);
+    
+    b' <@ A(OP, OR).distinguish();
+    
     return b';
   } 
 }.
 
-local lemma Pr_count &m b : 
-  hoare[ A(Wrapped_Oracle(ERO),RepO(Wrapped_Oracle(ERO))).distinguish : 
-     Wrapped_Oracle.ch = 0 /\ RepO.ctr = 0 /\ RepO.se 
-     ==> Wrapped_Oracle.ch <= query_ctr /\ 
-     RepO.ctr <= rep_ctr /\ RepO.se] 
-  =>
-  Pr[ReproGame(ERO,A).main(b) @ &m:res] = Pr[ReproGame(ERO,A).main(b) @ &m:res /\  Wrapped_Oracle.ch <= query_ctr /\ RepO.ctr <= rep_ctr /\ RepO.se].
+local lemma Pr_count &m (b : bool) : 
+     hoare[ A(O_Programmable(ERO),O_Reprogrammer(O_Programmable(ERO))).distinguish : 
+             O_Programmable.ch = 0 /\ O_Reprogrammer.ctr = 0 /\ O_Reprogrammer.se 
+             ==> O_Programmable.ch <= query_ctr /\ 
+             O_Reprogrammer.ctr <= rep_ctr /\ O_Reprogrammer.se] 
+  => Pr[IND_Repro(ERO, A).main(b) @ &m : res] 
+     = 
+     Pr[IND_Repro(ERO,A).main(b) @ &m : res /\ O_Programmable.ch <= query_ctr /\ O_Reprogrammer.ctr <= rep_ctr /\ O_Reprogrammer.se].
 proof.
-  move=> hhoare; byequiv => //.
-  conseq (: _ ==> ={res, Wrapped_Oracle.ch, RepO.ctr, RepO.se}) (: true ==> Wrapped_Oracle.ch <= query_ctr /\ RepO.ctr <= rep_ctr /\ RepO.se) _ => //; 2: by sim.
-  by proc; call hhoare; inline *; auto => /=.
+move=> hhoare.
+byequiv => //.
+conseq (: _ ==> ={res, O_Programmable.ch, O_Reprogrammer.ctr, O_Reprogrammer.se}) 
+       (: true ==> O_Programmable.ch <= query_ctr /\ O_Reprogrammer.ctr <= rep_ctr /\ O_Reprogrammer.se) 
+       _ => //; 2: by sim.
+by proc; call hhoare; inline *; auto => /=.
 qed.
 
 local lemma Pr_Game_Game1 &m b : 
-  Pr[ReproGame(ERO,A).main(b) @ &m:res /\  Wrapped_Oracle.ch <= query_ctr /\ RepO.ctr <= rep_ctr /\ RepO.se] =
-  Pr[ReproGame1(ERO,A).main(b) @ &m:res /\  Wrapped_Oracle.ch <= query_ctr /\ RepO.ctr <= rep_ctr /\ RepO.se].
+  Pr[IND_Repro(ERO,A).main(b) @ &m:res /\  O_Programmable.ch <= query_ctr /\ O_Reprogrammer.ctr <= rep_ctr /\ O_Reprogrammer.se] =
+  Pr[IND_Repro1(ERO,A).main(b) @ &m:res /\  O_Programmable.ch <= query_ctr /\ O_Reprogrammer.ctr <= rep_ctr /\ O_Reprogrammer.se].
 proof.
-  byequiv => //.
-  proc.
-  call (: ={glob ERO,  glob RepO, glob Wrapped_Oracle} /\ ((RepO.ctr, Wrapped_Oracle.ch) = (Bad.cr,Bad.co)){2} ).
-  + by proc; case: (Bad.co{2} < query_ctr); [rcondt{2} 2 | rcondf{2} 2]; auto => /=; conseq (: ={r}) => />; sim.
-  + proc. seq 1 1: (#pre); 1: by auto.
-    swap{1} 1 2.
-    by case: ((RepO.se /\ Bad.cr < rep_ctr){2}); [rcondt{2} 2 | rcondf{2} 2]; auto => /=; sim/>.
-  inline *; auto. swap{2} [1..3] 3; auto; sim />.
+byequiv => //.
+proc.
+call (:    ={glob ERO,  glob O_Reprogrammer, glob O_Programmable} 
+       /\ ((O_Reprogrammer.ctr, O_Programmable.ch) = (Bad.cr,Bad.co)){2}).
++ proc.
+  case (Bad.co{2} < query_ctr). 
+  - rcondt{2} 2; 1: by auto.
+    wp; conseq (: _ ==> ={r}) => //.
+    by inline *; wp; skip.
+  rcondf{2} 2; 1: by auto.
+  wp; conseq (: _ ==> ={r}) => //.
+  by inline *; wp; skip.
++ proc. 
+  seq 1 1: (#pre); 1: by auto.
+  swap{1} 1 2.
+  case ((O_Reprogrammer.se /\ Bad.cr < rep_ctr){2}).
+  + rcondt{2} 2; 1: by auto. 
+    by wp => />; sim.
+  rcondf{2} 2; 1: by auto. 
+  by wp => />; sim.
+inline *.
+wp.
+swap{2} [1..3] 3.
+by wp => />; sim.
 qed.
 
 local lemma Pr_Game1_Game2 &m b: 
-  Pr[ReproGame1(ERO,A).main(b) @ &m: res /\ Wrapped_Oracle.ch <= query_ctr /\ RepO.ctr <= rep_ctr /\ RepO.se] =
-  Pr[ReproGame2(ERO,A).main(b) @ &m: res /\ Wrapped_Oracle.ch <= query_ctr /\ RepO.ctr <= rep_ctr /\ RepO.se].
+  Pr[IND_Repro1(ERO,A).main(b) @ &m: res /\ O_Programmable.ch <= query_ctr /\ O_Reprogrammer.ctr <= rep_ctr /\ O_Reprogrammer.se] =
+  Pr[IND_Repro2(ERO,A).main(b) @ &m: res /\ O_Programmable.ch <= query_ctr /\ O_Reprogrammer.ctr <= rep_ctr /\ O_Reprogrammer.se].
 proof.
-  have : `|Pr[ReproGame1(ERO,A).main(b) @ &m: res /\ Wrapped_Oracle.ch <= query_ctr /\ RepO.ctr <= rep_ctr /\ RepO.se] -
-           Pr[ReproGame2(ERO,A).main(b) @ &m: res /\ Wrapped_Oracle.ch <= query_ctr /\ RepO.ctr <= rep_ctr /\ RepO.se] | <=
-         RealOrder.maxr Pr[ReproGame1(ERO,A).main(b) @ &m: (res /\ Wrapped_Oracle.ch <= query_ctr /\ RepO.ctr <= rep_ctr /\ RepO.se) /\ Bad.bad] 
-                        Pr[ReproGame2(ERO,A).main(b) @ &m: (res /\ Wrapped_Oracle.ch <= query_ctr /\ RepO.ctr <= rep_ctr /\ RepO.se) /\ Bad.bad].
-  + byupto.
-  have -> : Pr[ReproGame1(ERO, A).main(b) @ &m : (res /\ Wrapped_Oracle.ch <= query_ctr /\ RepO.ctr <= rep_ctr /\ RepO.se) /\ Bad.bad] = 0%r.
-  + byphoare => //; hoare.
-    proc. call (: Bad.cr <= RepO.ctr /\ Bad.co <= Wrapped_Oracle.ch /\ (Bad.bad => ! (Wrapped_Oracle.ch <= query_ctr /\ RepO.ctr <= rep_ctr /\ RepO.se))). 
-    + proc; sp; wp; if; auto; call (: true); auto => /#.
-    + proc; sp; wp; if; auto. 
-      + by conseq (: true); auto => /#.
-      by swap 1 2; wp; conseq (:true); auto => /#.
-    inline *; swap [1..3] 3; auto; conseq (: true) => //= /#.
-  have -> /#: Pr[ReproGame2(ERO, A).main(b) @ &m : (res /\ Wrapped_Oracle.ch <= query_ctr /\ RepO.ctr <= rep_ctr /\ RepO.se) /\ Bad.bad] = 0%r.
-  byphoare => //; hoare.
-  proc. call (: Bad.cr <= RepO.ctr /\ Bad.co <= Wrapped_Oracle.ch /\ (Bad.bad => ! (Wrapped_Oracle.ch <= query_ctr /\ RepO.ctr <= rep_ctr /\ RepO.se))). 
-  + by proc; sp; wp; if; auto; 1: call (: true); auto => /#.
-  + proc; sp; wp; if; auto; 2: smt().
-    by conseq (: true); auto => /#.
-  by inline *; swap [1..3] 3; auto; conseq (: true) => //= /#.
+have: 
+  `| Pr[IND_Repro1(ERO,A).main(b) @ &m: res /\ O_Programmable.ch <= query_ctr /\ O_Reprogrammer.ctr <= rep_ctr /\ O_Reprogrammer.se] -
+     Pr[IND_Repro2(ERO,A).main(b) @ &m: res /\ O_Programmable.ch <= query_ctr /\ O_Reprogrammer.ctr <= rep_ctr /\ O_Reprogrammer.se] | 
+  <=
+  RealOrder.maxr Pr[IND_Repro1(ERO,A).main(b) @ &m: (res /\ O_Programmable.ch <= query_ctr /\ O_Reprogrammer.ctr <= rep_ctr /\ O_Reprogrammer.se) /\ Bad.bad] 
+                 Pr[IND_Repro2(ERO,A).main(b) @ &m: (res /\ O_Programmable.ch <= query_ctr /\ O_Reprogrammer.ctr <= rep_ctr /\ O_Reprogrammer.se) /\ Bad.bad].
++ byupto.
+have ->: 
+  Pr[IND_Repro1(ERO, A).main(b) @ &m : (res /\ O_Programmable.ch <= query_ctr /\ O_Reprogrammer.ctr <= rep_ctr /\ O_Reprogrammer.se) /\ Bad.bad] 
+  = 
+  0%r.
++ byphoare => //.
+  hoare.
+  proc. 
+  call (:   Bad.cr <= O_Reprogrammer.ctr 
+          /\ Bad.co <= O_Programmable.ch 
+          /\ (Bad.bad => ! (O_Programmable.ch <= query_ctr /\ O_Reprogrammer.ctr <= rep_ctr /\ O_Reprogrammer.se))). 
+  + by proc; sp; wp; if; auto; call (: true); auto => /#.
+  + proc; sp; wp; if; auto. 
+    - by conseq (: _ ==> true); auto => /#.
+    by swap 1 2; wp; conseq (: _ ==> true); auto => /#.
+  inline *; swap [1..3] 3; auto; conseq (: _ ==> true) => //= /#.
+have -> /#: 
+  Pr[IND_Repro2(ERO, A).main(b) @ &m : (res /\ O_Programmable.ch <= query_ctr /\ O_Reprogrammer.ctr <= rep_ctr /\ O_Reprogrammer.se) /\ Bad.bad] 
+  = 
+  0%r.
+byphoare => //.
+hoare.
+proc. 
+call (:   Bad.cr <= O_Reprogrammer.ctr 
+       /\ Bad.co <= O_Programmable.ch 
+       /\ (Bad.bad => ! (O_Programmable.ch <= query_ctr /\ O_Reprogrammer.ctr <= rep_ctr /\ O_Reprogrammer.se))). 
++ by proc; sp; wp; if; auto; 1: call (: true); auto => /#.
++ proc; sp; wp; if; auto; 2: smt().
+  by conseq (: _ ==> true); auto => /#.
+by inline *; swap [1..3] 3; auto; conseq (: _ ==> true) => //= /#.
 qed.
 
-local module RepO2i : RepO_ti = {
-  include var RepO(Wrapped_Oracle2'(ERO)) [-repro]
+local module O_Reprogrammer2i : Oracleir_t = {
+  include var O_Reprogrammer(O_Programmable2S(ERO)) [-repro]
   import var Bad
 
   proc repro(p: pT) : in_t = {
-    var x,y;
+    var x : in_t;
+    var y : out_t;
+    
     se <- if p_max p <= p_max_bound then se else false;
+    
     x <- witness;
     if (se /\ cr < rep_ctr) { 
       x <$ p;
       if (i <= cr) {
         y <$ dout;
-        Wrapped_Oracle2(ERO).set(x,y);
+        O_Programmable2(ERO).set(x,y);
       }
       cr <- cr + 1;
     } 
+    
     ctr <- ctr + 1;
+    
     return x;
   }
 }.
 
 local module Hi = {
   import var Bad
-  module Wrap = Wrapped_Oracle2'(ERO)
-  module O = RepO2i
+  
+  module OP = O_Programmable2S(ERO)
+  module OR = O_Reprogrammer2i
  
   proc main (i0: int) : bool = {
-    var b';
+    var b' : bool;
+    
     bad <- false; cr <- 0; co <- 0; i <- i0;
+    
     ERO.init();
-    Wrap.init();
-    O.init(false);
-    b' <@ A(Wrap, O).distinguish();
-    return b' /\ Wrapped_Oracle.ch <= query_ctr /\ RepO.ctr <= rep_ctr /\ RepO.se;
+    OP.init();
+    OR.init(false);
+    
+    b' <@ A(OP, OR).distinguish();
+    
+    return b' /\ O_Programmable.ch <= query_ctr /\ O_Reprogrammer.ctr <= rep_ctr /\ O_Reprogrammer.se;
   } 
 }.
 
 local lemma Hi_true &m : 
-  Pr[ReproGame2(ERO, A).main(true) @ &m :
-       res /\ Wrapped_Oracle.ch <= query_ctr /\ RepO.ctr <= rep_ctr /\ RepO.se]  = 
+  Pr[IND_Repro2(ERO, A).main(true) @ &m : res /\ O_Programmable.ch <= query_ctr /\ O_Reprogrammer.ctr <= rep_ctr /\ O_Reprogrammer.se]
+  = 
   Pr[Hi.main(0) @ &m : res].
 proof.
-  byequiv => //; proc.
-  call (: ={glob Wrapped_Oracle, RepO.se, RepO.ctr, ERO.m, Bad.cr, Bad.co} /\ RepO.b{1} /\ (Bad.i <= Bad.cr){2}  ).
-  + by sim />.
-  + proc. 
-    seq 2 2 : (#pre /\ ={x}); 1: by auto.
-    wp; if; auto.
-    conseq (: ={glob Wrapped_Oracle, RepO.se, RepO.ctr, ERO.m, x}); 1: smt().
-    seq 1 1 : (#pre); 1: by sim />.
-    by if; auto; sim.
-  inline *; swap{1} [1 ..3] 3; swap{2} [1 ..4] 3; auto; sim />.
+byequiv => //.
+proc.
+call (:   ={glob O_Programmable, O_Reprogrammer.se, O_Reprogrammer.ctr, ERO.m, Bad.cr, Bad.co} 
+       /\ O_Reprogrammer.b{1} 
+       /\ (Bad.i <= Bad.cr){2}).
++ by sim />.
++ proc. 
+  seq 2 2 : (#pre /\ ={x}); 1: by auto.
+  wp; if; auto.
+  conseq (: ={glob O_Programmable, O_Reprogrammer.se, O_Reprogrammer.ctr, ERO.m, x}); 1: smt().
+  seq 1 1 : (#pre); 1: by sim />.
+  by if; auto; sim.
+by inline *; swap{1} [1 ..3] 3; swap{2} [1 ..4] 3; auto; sim />.
 qed.
 
 local lemma Hi_false &m : 
-  Pr[ReproGame2(ERO, A).main(false) @ &m :
-       res /\ Wrapped_Oracle.ch <= query_ctr /\ RepO.ctr <= rep_ctr /\ RepO.se]  = 
+  Pr[IND_Repro2(ERO, A).main(false) @ &m : res /\ O_Programmable.ch <= query_ctr /\ O_Reprogrammer.ctr <= rep_ctr /\ O_Reprogrammer.se]
+  = 
   Pr[Hi.main(rep_ctr) @ &m : res].
 proof.
-  byequiv => //; proc.
-  call (: ={glob Wrapped_Oracle, RepO.se, RepO.ctr, ERO.m, Bad.cr, Bad.co} /\ !RepO.b{1} /\ (Bad.i = rep_ctr){2}).
-  + by sim />.
-  + proc. 
-    seq 2 2 : (#pre /\ ={x}); 1: by auto.
-    wp; if; auto.
-    rcondf{1} ^if; 1: by auto.
-    by rcondf{2} ^if; auto => /#.
-  inline *; swap{1} [1 ..3] 3; swap{2} [1 ..4] 3; auto; sim />.
+byequiv => //.
+proc.
+call (:   ={glob O_Programmable, O_Reprogrammer.se, O_Reprogrammer.ctr, ERO.m, Bad.cr, Bad.co} 
+       /\ !O_Reprogrammer.b{1} 
+       /\ (Bad.i = rep_ctr){2}).
++ by sim />.
++ proc. 
+  seq 2 2 : (#pre /\ ={x}); 1: by auto.
+  wp; if; auto.
+  rcondf{1} ^if; 1: by auto.
+  by rcondf{2} ^if; auto => /#.
+inline *; swap{1} [1 ..3] 3; swap{2} [1 ..4] 3; auto; sim />.
 qed.
 
-local module RepO2i1 (RO: POracle) : RepO_ti = {
+local module O_Reprogrammer2i1 (O: POracle) : Oracleir_t = {
   import var Bad
 
-  include var RepO(Wrapped_Oracle2'(RO)) [-repro]
+  include var O_Reprogrammer(O_Programmable2S(O)) [-repro]
   
   var x_ : in_t
 
   proc repro(p: pT) : in_t = {
-    var x,y;
+    var x : in_t;
+    var y : out_t;
+    
     se <- if p_max p <= p_max_bound then se else false;
+    
     x <- witness;
     if (se /\ cr < rep_ctr) { 
       x <$ p;
       if (i + 1 <= cr) {
         y <$ dout;
-        Wrapped_Oracle2'(RO).set(x,y);
+        O_Programmable2S(O).set(x,y);
       } else { 
         if (i = cr) {
           x_ <- x;
-          y <@ RO.o(x);
+          y <@ O.o(x);
         } 
       } 
       cr <- cr + 1;
     } 
+    
     ctr <- ctr + 1;
+    
     return x;
   }
 }.
 
-local module Hi1 (RO:POracle) = {
+local module Hi1 (O:POracle) = {
   import var Bad
-  module Wrap = Wrapped_Oracle2'(RO)
-  module O = RepO2i1(RO)
+  
+  module OP = O_Programmable2S(O)
+  module OR = O_Reprogrammer2i1(O)
  
   proc run (i0: int) : bool = {
-    var b';
+    var b' : bool;
+ 
     bad <- false;  cr <- 0; co <- 0; i <- i0;
-    Wrap.init();
-    O.init(false);
-    b' <@ A(Wrap, O).distinguish();
-    return b' /\ Wrapped_Oracle.ch <= query_ctr /\ RepO.ctr <= rep_ctr /\ RepO.se;
+    OP.init();
+    OR.init(false);
+ 
+    b' <@ A(OP, OR).distinguish();
+ 
+    return b' /\ O_Programmable.ch <= query_ctr /\ O_Reprogrammer.ctr <= rep_ctr /\ O_Reprogrammer.se;
   } 
 }.
 
-local lemma Hip1_Hi1 &m i_ : Pr[Hi.main(i_ + 1) @ &m : res] = Pr[ Exp(ERO, Hi1).main(i_) @ &m : res].
+local lemma Hip1_Hi1 &m i_ : 
+  Pr[Hi.main(i_ + 1) @ &m : res] 
+  = 
+  Pr[Exp(ERO, Hi1).main(i_) @ &m : res].
 proof.
-  byequiv => //; proc; inline *; wp.
-  call (: ={ERO.m, glob Wrapped_Oracle, glob RepO, Bad.cr, Bad.co} /\ Bad.i{1} = Bad.i{2} + 1).
-  + by sim />.
-  + proc; wp; conseq />.
-    seq 2 2 : (#pre /\ ={x}); 1: by auto.
-    if => //.
-    seq 1 1 : (#pre); 1: by auto.
-    if => //; 1: by sim.
-    by inline *; auto.
-  swap{1} [1..4] 3; auto; sim />.
+byequiv => //. 
+proc. 
+inline *; wp.
+call (:   ={ERO.m, glob O_Programmable, glob O_Reprogrammer, Bad.cr, Bad.co} 
+       /\ Bad.i{1} = Bad.i{2} + 1).
++ by sim />.
++ proc; wp; conseq />.
+  seq 2 2 : (#pre /\ ={x}); 1: by auto.
+  if => //.
+  seq 1 1 : (#pre); 1: by auto.
+  if => //; 1: by sim.
+  by inline *; auto.
+by swap{1} [1..4] 3; auto; sim />.
 qed.
 
-local lemma Hi1_ERO_LRO  &m i_ : Pr[ Exp(ERO,Hi1).main(i_) @ &m : res] = Pr[ Exp(Lazy.LRO,Hi1).main(i_) @ &m : res].
+local lemma Hi1_ERO_LRO  &m i_ : 
+  Pr[Exp(ERO,Hi1).main(i_) @ &m : res] 
+  =
+  Pr[Exp(Lazy.LRO,Hi1).main(i_) @ &m : res].
 proof.
-  byequiv (: ={glob Hi1, arg} ==> ={res}) => //; symmetry.
-  conseq (eq_eager_sampling Hi1 _) => // *; apply dout_ll.
+byequiv (: ={glob Hi1, arg} ==> ={res}) => //; symmetry.
+conseq (eq_eager_sampling Hi1 _) => // *; apply dout_ll.
 qed.
 
-local module RepO2i2 : RepO_ti = {
+local module O_Reprogrammer2i2 : Oracleir_t = {
   import var Bad
-  include var RepO(Wrapped_Oracle2'(Lazy.LRO)) [-repro]
+  include var O_Reprogrammer(O_Programmable2S(Lazy.LRO)) [-repro]
+  
   var x_ : in_t
 
   proc repro(p : pT) : in_t = {
-    var x,y;
+    var x : in_t;
+    var y : out_t;
+    
     se <- if p_max p <= p_max_bound then se else false;
+    
     x <- witness;
     if (se /\  cr < rep_ctr) { 
       x <$ p;
       if (i + 1 <= cr) {
         y <$ dout;
-        Wrapped_Oracle2'(Lazy.LRO).set(x,y);
+        O_Programmable2S(Lazy.LRO).set(x,y);
       } else { if (i = cr /\ fsize Lazy.LRO.m <= query_ctr) {
         x_ <- x;
         if (! x \in Lazy.LRO.m) {
@@ -498,42 +605,52 @@ local module RepO2i2 : RepO_ti = {
       } } 
       cr <- cr + 1;
     } 
+    
     ctr <- ctr + 1;
+    
     return x;
   }
 }.
 
 local module Hi2 = {
   import var Bad
-  module Wrap = Wrapped_Oracle2'(Lazy.LRO)
-  module O = RepO2i2
+  
+  module OP = O_Programmable2S(Lazy.LRO)
+  module OR = O_Reprogrammer2i2
  
   proc run (i0: int) : bool = {
-    var b';
+    var b' : bool;
+    
     bad <- false;  cr <- 0; co <- 0; i <- i0;
+    
     Lazy.LRO.init();
-    Wrap.init();
-    O.init(false);
-    b' <@ A(Wrap, O).distinguish();
-    return b' /\ Wrapped_Oracle.ch <= query_ctr /\ RepO.ctr <= rep_ctr /\ RepO.se;
+    OP.init();
+    OR.init(false);
+    
+    b' <@ A(OP, OR).distinguish();
+    
+    return b' /\ O_Programmable.ch <= query_ctr /\ O_Reprogrammer.ctr <= rep_ctr /\ O_Reprogrammer.se;
   } 
 }.
 
-local module RepO2i3 : RepO_ti = {
+local module O_Reprogrammer2i3 : Oracleir_t = {
   import var Bad
-  include var RepO(Wrapped_Oracle2'(Lazy.LRO)) [-repro]
+  include var O_Reprogrammer(O_Programmable2S(Lazy.LRO)) [-repro]
 
   proc repro(p: pT) : in_t = {
-    var x,y;
+    var x : in_t;
+    var y : out_t;
+
     se <- if p_max p <= p_max_bound then se else false;
+    
     x <- witness;
     if (se /\ cr < rep_ctr) { 
       x <$ p;
       if (i + 1 <= cr) {
         y <$ dout;
-        Wrapped_Oracle2'(Lazy.LRO).set(x,y);
+        O_Programmable2S(Lazy.LRO).set(x,y);
       } else { if (i = cr /\ fsize Lazy.LRO.m <= query_ctr) {
-        RepO2i2.x_ <- x;
+        O_Reprogrammer2i2.x_ <- x;
         if (! x \in Lazy.LRO.m) {
           y <@ Lazy.LRO.o(x);
         } else { 
@@ -544,54 +661,74 @@ local module RepO2i3 : RepO_ti = {
       } } 
       cr <- cr + 1;
     } 
+
     ctr <- ctr + 1;
+    
     return x;
   }
 }.
 
 local module Hi3 = {
   import var Bad
-  module Wrap = Wrapped_Oracle2'(Lazy.LRO)
-  module O = RepO2i3
+  
+  module OP = O_Programmable2S(Lazy.LRO)
+  module OR = O_Reprogrammer2i3
  
   proc run (i0: int) : bool = {
     var b';
     
     bad <- false;  cr <- 0; co <- 0; i <- i0;
+  
     Lazy.LRO.init();
-    Wrap.init();
-    O.init(false);
-    b' <@ A(Wrap, O).distinguish();
-    return b' /\ Wrapped_Oracle.ch <= query_ctr /\ RepO.ctr <= rep_ctr /\ RepO.se;
+    OP.init();
+    OR.init(false);
+  
+    b' <@ A(OP, OR).distinguish();
+  
+    return b' /\ O_Programmable.ch <= query_ctr /\ O_Reprogrammer.ctr <= rep_ctr /\ O_Reprogrammer.se;
   } 
 }.
 
 local lemma Hi1_LRO_Hi2  &m i_ : Pr[ Exp(Lazy.LRO,Hi1).main(i_) @ &m : res] = Pr[Hi2.run(i_) @ &m : res].
 proof.
-  byequiv => //; proc; inline *; wp.
-  call (: ={ Lazy.LRO.m, glob Wrapped_Oracle, glob RepO, Bad.cr, Bad.co, Bad.i} /\ (Bad.cr <= Bad.i => fsize Lazy.LRO.m <= Bad.co <= query_ctr){1}); last first.
-  + by auto => />; rewrite fsize_empty ge0_queryctr.
-  + by proc; sp; inline *; if; auto => /> &2 3? r *; rewrite fsize_set /b2i => /> /#.
-  proc; wp; seq 2 2 : (#pre /\ ={x}); 1: by sim />.
-  if => //.  
-  seq 1 1: (#pre); 1: by sim />.
-  if => //.
-  + by wp; conseq (: ={y, Wrapped_Oracle.prog_list});[ smt() | sim].
-  wp; if => //; 1: smt().
-  + by sp 1 1; conseq (: ={Lazy.LRO.m}); [smt() | if{2}; sim].
-  auto => /#.
+byequiv => //.
+proc. 
+inline *; wp.
+call (:   ={ Lazy.LRO.m, glob O_Programmable, glob O_Reprogrammer, Bad.cr, Bad.co, Bad.i} 
+       /\ (Bad.cr <= Bad.i => fsize Lazy.LRO.m <= Bad.co <= query_ctr){1}); last first.
++ by auto => />; rewrite fsize_empty ge0_queryctr.
++ by proc; sp; inline *; if; auto => /> &2 3? r *; rewrite fsize_set /b2i => /> /#.
+proc. 
+wp. 
+seq 2 2 : (#pre /\ ={x}); 1: by sim />.
+if => //.  
+seq 1 1: (#pre); 1: by sim />.
+if => //.
++ wp. 
+  by conseq (: _ ==> ={y, O_Programmable.prog_list}); [smt() | sim].
+wp. 
+if => //; 1: smt().
++ sp 1 1. 
+  conseq (: _ ==> ={Lazy.LRO.m}); [smt() | if{2}; sim].
+by auto => /#.
 qed.
 
 local lemma Hi2_Hi3 &m i_ : 
-  `|Pr[ Hi2.run(i_) @ &m : res] - Pr[Hi3.run(i_) @ &m : res]| <=
-   maxr Pr[ Hi2.run(i_) @ &m : Bad.bad] Pr[ Hi3.run(i_) @ &m : Bad.bad].
+  `| Pr[ Hi2.run(i_) @ &m : res] - Pr[Hi3.run(i_) @ &m : res] | 
+  <=
+  maxr Pr[ Hi2.run(i_) @ &m : Bad.bad] Pr[ Hi3.run(i_) @ &m : Bad.bad].
 proof. byupto. qed.
 
 local lemma Hi2_bad &m i_ : 0 <= i_ => Pr[ Hi2.run(i_) @ &m : Bad.bad] <= query_ctr%r * p_max_bound.
 proof.
-move=> hi; fel 4 (b2i (Bad.i < Bad.cr)) (fun x => query_ctr%r * p_max_bound) 1 Bad.bad
-  [RepO2i2.repro : ((if p_max p <= p_max_bound then RepO.se else false) /\ Bad.cr < rep_ctr /\
-                      Bad.i = Bad.cr /\ fsize Lazy.LRO.m <= query_ctr)] => //.
+move=> hi.
+fel 4 
+    (b2i (Bad.i < Bad.cr)) 
+    (fun x => query_ctr%r * p_max_bound) 
+    1 
+    Bad.bad
+    [O_Reprogrammer2i2.repro :   ((if p_max p <= p_max_bound then O_Reprogrammer.se else false) 
+                              /\ Bad.cr < rep_ctr /\ Bad.i = Bad.cr /\ fsize Lazy.LRO.m <= query_ctr)] => //.
 + by rewrite sumri_const.
 + smt().
 + auto => /> /#.
@@ -609,24 +746,35 @@ move=> hi; fel 4 (b2i (Bad.i < Bad.cr)) (fun x => query_ctr%r * p_max_bound) 1 B
     apply: Mu_mem.mu_mem_le_fsize.
     + move=> x hx /=; apply: ler_trans hmax; move: (pmax_upper_bound p{hr} x) => /#.
     by apply ler_wpmul2r; smt(pmax_ge0). 
-  by rcondt ^if; auto; conseq (: false).
-+ move=> c;proc.
+  by rcondt ^if; auto; conseq (: _ ==> false).
++ move=> c.
+  proc.
   rcondt ^if; 1: by auto.
-  by wp; conseq (: true) => //; smt().
+  by wp; conseq (: _ ==> true) => //; smt().
 move=> b c; proc.
-seq 2: (! (RepO.se /\ Bad.cr < rep_ctr /\ Bad.i = Bad.cr /\ FSet.card (fdom Lazy.LRO.m) <= query_ctr) /\
-             Bad.bad = b /\ b2i (Bad.i < Bad.cr) = c); 1: by auto.
+seq 2: (   ! (O_Reprogrammer.se /\ Bad.cr < rep_ctr /\ Bad.i = Bad.cr /\ FSet.card (fdom Lazy.LRO.m) <= query_ctr) 
+        /\ Bad.bad = b 
+        /\ b2i (Bad.i < Bad.cr) = c); 1: by auto.
 wp; if; last by auto.
 seq 1 : (#pre); 1: by auto.
-wp; if; 1: by conseq (:true) => // /#.
-rcondf ^if; auto => /#. 
+wp; if; 1: by conseq (: _ ==> true) => // /#.
+by rcondf ^if; auto => /#. 
 qed.
 
-local lemma Hi3_bad &m i_ :  0 <= i_ => Pr[ Hi3.run(i_) @ &m : Bad.bad] <= query_ctr%r * p_max_bound.
+local lemma Hi3_bad &m i_ :
+     0 <= i_ 
+  => Pr[ Hi3.run(i_) @ &m : Bad.bad] 
+     <= 
+     query_ctr%r * p_max_bound.
 proof.
-move=> hi; fel 4 (b2i (Bad.i < Bad.cr)) (fun x => query_ctr%r * p_max_bound) 1 Bad.bad
-  [RepO2i3.repro : ((if p_max p <= p_max_bound then RepO.se else false) /\ Bad.cr < rep_ctr /\
-                      Bad.i = Bad.cr /\ fsize Lazy.LRO.m <= query_ctr)] => //.
+move=> hi.
+fel 4 
+    (b2i (Bad.i < Bad.cr)) 
+    (fun x => query_ctr%r * p_max_bound) 
+    1 
+    Bad.bad
+    [O_Reprogrammer2i3.repro :   ((if p_max p <= p_max_bound then O_Reprogrammer.se else false) 
+                              /\ Bad.cr < rep_ctr /\ Bad.i = Bad.cr /\ fsize Lazy.LRO.m <= query_ctr)] => //.
 + by rewrite sumri_const.
 + smt().
 + auto => /> /#.
@@ -636,7 +784,7 @@ move=> hi; fel 4 (b2i (Bad.i < Bad.cr)) (fun x => query_ctr%r * p_max_bound) 1 B
   rcondt ^if; 1: by auto.
   wp; seq 3 : (x \in Lazy.LRO.m) (query_ctr%r * p_max_bound) 1%r _ 0%r (!Bad.bad) => //.
   + by auto.
-  + rnd (fun p  => p \in Lazy.LRO.m); auto.
+  + rnd; auto.
     move=> &hr /> _ _ _ hmax _ _ hsz.
     apply (ler_trans (mu p{hr} (fun (p0 : in_t) => exists x, dom Lazy.LRO.m{hr} x /\ x = p0))).
     + by apply mu_le => /> x0 *; exists x0.
@@ -644,114 +792,148 @@ move=> hi; fel 4 (b2i (Bad.i < Bad.cr)) (fun x => query_ctr%r * p_max_bound) 1 B
     apply: Mu_mem.mu_mem_le_fsize.
     + by move=> x hx /=; apply: ler_trans hmax;  move: (pmax_upper_bound p{hr} x) => /#.
     by apply ler_wpmul2r; smt(pmax_ge0). 
-  by rcondt ^if; auto; conseq (: false).
-+ move=> c;proc.
+  by rcondt ^if; auto; conseq (: _ ==> false).
++ move=> c.
+  proc.
   rcondt ^if; 1: by auto.
-  by wp; conseq (: true) => //; smt().
-move=> b c; proc.
-seq 2: (! (RepO.se /\ Bad.cr < rep_ctr /\ Bad.i = Bad.cr /\ FSet.card (fdom Lazy.LRO.m) <= query_ctr) /\
+  by wp; conseq (: _ ==> true) => //; smt().
+move=> b c. 
+proc.
+seq 2: (! (O_Reprogrammer.se /\ Bad.cr < rep_ctr /\ Bad.i = Bad.cr /\ FSet.card (fdom Lazy.LRO.m) <= query_ctr) /\
              Bad.bad = b /\ b2i (Bad.i < Bad.cr) = c); 1: by auto.
 wp; if; last by auto.
 seq 1 : (#pre); 1: by auto.
-wp; if; 1: by conseq (:true) => // /#.
-rcondf ^if; auto => /#.
+wp; if; 1: by conseq (: _ ==> true) => // /#.
+by rcondf ^if; auto => /#.
 qed.
 
-local module RepO2i4 (RO: POracle) : RepO_ti = {
+local module O_Reprogrammer2i4 (O: POracle) : Oracleir_t = {
   import var Bad
-  include var RepO(Wrapped_Oracle2'(RO)) [-repro]
+  include var O_Reprogrammer(O_Programmable2S(O)) [-repro]
+  
   var x_ : in_t
 
   proc repro(p: pT) : in_t = {
-    var x,y;
+    var x : in_t;
+    var y : out_t;
+    
     se <- if p_max p <= p_max_bound then se else false;
+    
     x <- witness;
     if (se /\ cr < rep_ctr) { 
       x <$ p;
       if (i <= cr) {
         y <$ dout;
-        Wrapped_Oracle2'(RO).set(x,y);
+        O_Programmable2S(O).set(x,y);
       }
       cr <- cr + 1;
     } 
+    
     ctr <- ctr + 1;
+    
     return x;
   }
 }.
 
-local module Hi4 (RO:POracle) = {
+local module Hi4 (O:POracle) = {
   import var Bad
-  module Wrap = Wrapped_Oracle2'(RO)
-  module O = RepO2i4(RO)
+  
+  module OP = O_Programmable2S(O)
+  module OR = O_Reprogrammer2i4(O)
  
   proc run (i0: int) : bool = {
-    var b';
+    var b' : bool;
+    
     bad <- false;  cr <- 0; co <- 0; i <- i0;
-    Wrap.init();
-    O.init(false);
-    b' <@ A(Wrap, O).distinguish();
-    return b' /\ Wrapped_Oracle.ch <= query_ctr /\ RepO.ctr <= rep_ctr /\ RepO.se;
+    
+    OP.init();
+    OR.init(false);
+    
+    b' <@ A(OP, OR).distinguish();
+    
+    return b' /\ O_Programmable.ch <= query_ctr /\ O_Reprogrammer.ctr <= rep_ctr /\ O_Reprogrammer.se;
   } 
 }.
 
-local lemma Hi3_Hi4 &m i_: 0 <= i_ => Pr[Hi3.run(i_) @ &m : res] = Pr[Exp(Lazy.LRO, Hi4).main(i_) @ &m : res].
+local lemma Hi3_Hi4 &m i_: 
+     0 <= i_ 
+  => Pr[Hi3.run(i_) @ &m : res] 
+     = 
+     Pr[Exp(Lazy.LRO, Hi4).main(i_) @ &m : res].
 proof.
-  move=> hi; byequiv => //; proc; inline *; wp.
-  call (: ={Wrapped_Oracle.ch, glob RepO, Bad.i, Bad.cr, Bad.co} /\ 
-     if (Bad.cr <= Bad.i){1} then ={Lazy.LRO.m, Wrapped_Oracle.prog_list} /\ Wrapped_Oracle.prog_list{1} = [] /\ (fsize Lazy.LRO.m <= Bad.co <= query_ctr){1}
-     else 
-       ((RepO2i2.x_ \in Lazy.LRO.m){1} /\
-        Wrapped_Oracle.prog_list{2} = (rcons Wrapped_Oracle.prog_list (RepO2i2.x_, oget Lazy.LRO.m.[RepO2i2.x_])){1} /\
-        eq_except (pred1 RepO2i2.x_{1}) Lazy.LRO.m{1} Lazy.LRO.m{2})).
-  + proc; sp; wp; if => //.
-    inline *; auto => |> &1 &2. 
-    case: (Bad.cr{2} <= Bad.i{2}) => |> 4? r ?.
-    + by rewrite fsize_set /b2i => /> /#.
-    rewrite -!cats1 assoc_cat.
-    by case: (assocP  Wrapped_Oracle.prog_list{1} x{2}) => />; smt(mem_set get_setE).
-  + proc; wp; seq 2 2 : (#pre /\ ={x}); 1: by auto.
-    if => //.
-    seq 1 1: (#pre /\ ={x}); 1: by auto.
-    if{1}.
-    + rcondt{2} ^if; 1: by auto => /#.
-      by inline *; auto => />; smt().
-    if{1}.
-    + rcondt{2} ^if; 1: by auto.
-      by sp 1 0; inline *; if{1}; auto; smt(get_setE remE).  
-    by rcondf{2} ^if; auto => /> /#. 
-  by auto => />; rewrite fsize_empty ge0_queryctr.
+move=> hi. 
+byequiv => //. 
+proc.
+inline *; wp.
+call (:   ={O_Programmable.ch, glob O_Reprogrammer, Bad.i, Bad.cr, Bad.co} 
+       /\ if (Bad.cr <= Bad.i){1} 
+          then    ={Lazy.LRO.m, O_Programmable.prog_list} 
+               /\ O_Programmable.prog_list{1} = [] 
+               /\ (fsize Lazy.LRO.m <= Bad.co <= query_ctr){1}
+          else    ((O_Reprogrammer2i2.x_ \in Lazy.LRO.m){1} 
+               /\ O_Programmable.prog_list{2} = (rcons O_Programmable.prog_list (O_Reprogrammer2i2.x_, oget Lazy.LRO.m.[O_Reprogrammer2i2.x_])){1} 
+               /\ eq_except (pred1 O_Reprogrammer2i2.x_{1}) Lazy.LRO.m{1} Lazy.LRO.m{2})).
++ proc.
+  sp; wp; if => //.
+  inline *; auto => |> &1 &2. 
+  case: (Bad.cr{2} <= Bad.i{2}) => |> 4? r ?.
+  + by rewrite fsize_set /b2i => /> /#.
+  rewrite -!cats1 assoc_cat.
+  by case: (assocP O_Programmable.prog_list{1} x{2}) => />; smt(mem_set get_setE).
++ proc. 
+  wp; seq 2 2 : (#pre /\ ={x}); 1: by auto.
+  if => //.
+  seq 1 1: (#pre /\ ={x}); 1: by auto.
+  if{1}.
+  + rcondt{2} ^if; 1: by auto => /#.
+    by inline *; auto => />; smt().
+  if{1}.
+  + rcondt{2} ^if; 1: by auto.
+    by sp 1 0; inline *; if{1}; auto; smt(get_setE remE).  
+  by rcondf{2} ^if; auto => /> /#. 
+  conseq />; 1: by smt().
+by auto => />; rewrite fsize_empty ge0_queryctr.
 qed.
 
-local lemma Hi4_LRO_ERO &m i_: Pr[Exp(Lazy.LRO, Hi4).main(i_) @ &m : res] = Pr[Exp(ERO, Hi4).main(i_) @ &m : res].
+local lemma Hi4_LRO_ERO &m i_: 
+  Pr[Exp(Lazy.LRO, Hi4).main(i_) @ &m : res] 
+  = 
+  Pr[Exp(ERO, Hi4).main(i_) @ &m : res].
 proof.
-  byequiv (: ={glob Hi4, arg} ==> ={res}) => //.
-  conseq (eq_eager_sampling Hi4 _) => // *;apply dout_ll.
+byequiv (: ={glob Hi4, arg} ==> ={res}) => //.
+by conseq (eq_eager_sampling Hi4 _) => // *; apply dout_ll.
 qed.
 
-local lemma Hi4_Hi &m i_ : Pr[Exp(ERO, Hi4).main(i_) @ &m : res] = Pr[Hi.main(i_) @ &m : res].
-proof. byequiv => //; proc; inline *; wp; swap{2} [1 .. 4] 3; sim. qed.
+local lemma Hi4_Hi &m i_ : 
+  Pr[Exp(ERO, Hi4).main(i_) @ &m : res] 
+  = 
+  Pr[Hi.main(i_) @ &m : res].
+proof. by byequiv => //; proc; inline *; wp; swap{2} [1 .. 4] 3; sim. qed.
 
-local lemma rom_reprogramming1 &m i_ : 0 <= i_ => 
-  `|Pr[Hi.main(i_ + 1) @ &m : res] - Pr[Hi.main(i_) @ &m : res]| <= query_ctr%r * p_max_bound.
+local lemma rom_reprogramming1 &m i_ : 
+     0 <= i_ 
+  => `| Pr[Hi.main(i_ + 1) @ &m : res] - Pr[Hi.main(i_) @ &m : res] | 
+     <= 
+     query_ctr%r * p_max_bound.
 proof.
-  move=> hi; rewrite (Hip1_Hi1 &m i_) (Hi1_ERO_LRO  &m i_) (Hi1_LRO_Hi2 &m i_).
-  rewrite -(Hi4_Hi &m i_) -(Hi4_LRO_ERO &m i_) -(Hi3_Hi4 &m i_) 1://.
-  move: (Hi2_Hi3 &m i_) (Hi2_bad &m i_) (Hi3_bad &m i_) => /#.
+move=> hi; rewrite (Hip1_Hi1 &m i_) (Hi1_ERO_LRO  &m i_) (Hi1_LRO_Hi2 &m i_).
+rewrite -(Hi4_Hi &m i_) -(Hi4_LRO_ERO &m i_) -(Hi3_Hi4 &m i_) 1://.
+by move: (Hi2_Hi3 &m i_) (Hi2_bad &m i_) (Hi3_bad &m i_) => /#.
 qed.
 
 (* ----------------------------------------------------- *)
 
-lemma rom_reprogramming &m : 
-   hoare[A(Wrapped_Oracle(ERO), RepO(Wrapped_Oracle(ERO))).distinguish : 
-     Wrapped_Oracle.ch = 0 /\ RepO.ctr = 0 /\ RepO.se 
-     ==> Wrapped_Oracle.ch <= query_ctr /\ 
-     RepO.ctr <= rep_ctr /\ RepO.se]
-  =>
- `|Pr[ReproGame(ERO, A).main(false) @ &m:res]
- - Pr[ReproGame(ERO, A).main(true) @ &m:res]|
-  <= rep_ctr%r * query_ctr%r * p_max_bound. 
+lemma Bound_IND_Repro &m : 
+     hoare[A(O_Programmable(ERO), O_Reprogrammer(O_Programmable(ERO))).distinguish : 
+             O_Programmable.ch = 0 /\ O_Reprogrammer.ctr = 0 /\ O_Reprogrammer.se 
+             ==> O_Programmable.ch <= query_ctr /\ 
+             O_Reprogrammer.ctr <= rep_ctr /\ O_Reprogrammer.se]
+  => `| Pr[IND_Repro(ERO, A).main(false) @ &m : res]
+       - Pr[IND_Repro(ERO, A).main(true) @ &m : res] |
+      <= 
+      rep_ctr%r * query_ctr%r * p_max_bound. 
 proof.
-move => Hquery.
+move=> Hquery.
 rewrite 2!(Pr_count &m _ Hquery) 2!(Pr_Game_Game1 &m) 2!(Pr_Game1_Game2 &m).
 rewrite Hi_true Hi_false.
 rewrite (telescoping_sum_down (fun i => Pr[Hi.main(i) @ &m : res]) 0 rep_ctr ge0_repctr) /=.
